$1.111 D$
$A \in \mathbb{R}^{m n} \forall b \in \mathbb{R}^{n}, A x^{2} b$ 有解 $\geqslant P(A)=m$

$$
R(A, b)=R^{(A)}
$$

$A:$ 如 $A=\left[L \mid \alpha_{1} \alpha_{l}\right]_{\alpha=\alpha}$
B）：$\quad A^{\top} \in R^{\text {mam }}$
$\forall d \quad A^{\prime} x=d$ 有解 2$) R(A)=n$
C．$A=\left(\begin{array}{lll}\alpha_{1} & \cdots & \alpha_{n}\end{array}\right)\left(\begin{array}{l}x_{i} \\ \vdots \\ \chi_{n}\end{array}\right)=\sum_{i=1}^{n} \alpha_{i} x_{i}$
D．$A \in \mid \mathbb{R}^{m \times n}$
![](https://cdn.mathpix.com/cropped/2025_04_10_fc620acbb4a35583838ag-01.jpg?height=408&width=2130&top_left_y=3443&top_left_x=954)
![](https://cdn.mathpix.com/cropped/2025_04_10_fc620acbb4a35583838ag-01.jpg?height=345&width=1739&top_left_y=3960&top_left_x=1009)
![](https://cdn.mathpix.com/cropped/2025_04_10_fc620acbb4a35583838ag-01.jpg?height=1003&width=4994&top_left_y=4116&top_left_x=1009)
（2）$A$ ．

$$
\begin{aligned}
& A: A x=0 \Rightarrow E A x=0=B x \\
& B: \operatorname{kn} A=\left[\begin{array}{lll}
1 & 1 & 0
\end{array}\right] \quad B\left[\begin{array}{cc}
1 & 1 \\
-1 & 0
\end{array}\right]
\end{aligned}
$$

（．$\quad A^{\top} x=0 \Leftrightarrow B^{\top} x=0(z) A^{\top} E^{\top} x=0$ ？

$$
\begin{gathered}
x \neq E^{\top} x \\
D: B^{\top} B=A^{\top} E^{\top} L^{2} A=A^{\top} A ? x
\end{gathered}
$$

（3）$B$
A：A：Nut symmetic．
B：$A x=0 \Leftrightarrow A^{\top} A x=0$
$C$ ：不能道意行变换
D：$n>m$ ．
14) $C$

Hint: $C=(A B)^{-1}=B^{-1} A^{-1}$
(5) C

$$
\begin{aligned}
& A=A^{2} \Rightarrow 0: A(A-L) \\
& \therefore R(A) \quad P R(A-I) \leq n \\
& 又 R(A)+R(B) \geqslant R(A+B) \\
& \text { 取 } 3=I-A \\
& R(A)+R(Z-A) \geqslant R(Z)=n
\end{aligned}
$$

2. (1) $\left[\begin{array}{ccc}1 & -\frac{1}{i} & -\frac{1}{6} \\ & \frac{1}{2} & -\frac{1}{6} \\ & & \frac{6}{3}\end{array}\right]$
(2) $\left[\begin{array}{lll}1 & & \\ 2 & 1 & \\ 3 & 1 & 1\end{array}\right]$
（3）$\frac{1}{14}\left[\begin{array}{lll}4 & 6 & 2 \\ 6 & 9 & 3 \\ 2 & 3 & 1\end{array}\right]$

投影到 $V, V$ besis：$V_{1} \ldots . . V_{m}$
$A:\left[v_{1} \ldots v_{m}\right]$

$$
P_{v}=A\left(A^{\top} A\right)^{-1} A^{\top}
$$

（4） 10

$$
\begin{aligned}
& A \in \mathbb{R}^{m \times n} \\
& N(A)=n-R(A) \\
& C(A)=K(A) \\
& C\left(A^{\top}\right)=R(A) \\
& \left.N(A)^{\top}\right)=m-R(A) \\
& m=2.24, \quad n=2025
\end{aligned}
$$

$$
\begin{aligned}
& \text { 3. (a) } l-A=\left[\begin{array}{ccc}
1 & -1 & 0 \\
-1 & 1 & 1 \\
0 & -1 & 1
\end{array}\right] \\
& l-A^{2}=\left[\begin{array}{ccc}
0 & 0 & 1 \\
0 & 1 & 0 \\
-1 & 0 & 2
\end{array}\right] \\
& X-X A^{2}-A X+A X A^{2}=I \\
& (Z-A) X\left(I-A^{2}\right)=I \\
& \left.X=(Z-A)^{-1}\left(I-A^{2}\right)^{-1}=\left[\left(I-A^{2}\right)(I-A)\right)\right]^{-1}=\left[\begin{array}{lll}
1 & 1 & -2 \\
1 & 1 & -1 \\
2 & 1 & -1
\end{array}\right]
\end{aligned}
$$

4．（a）$\left[\begin{array}{lll}1 & 0 & 2 \\ 0 \\ 0 & 0 & 1 \\ 0 & 0 \\ 0 & 0 & 0 \\ 0 & 0 & 0 \\ 0\end{array}\right]$ Pinuts 上分均为0！
（b）

$$
\begin{aligned}
& c(A)=k_{1}\left[\begin{array}{l}
1 \\
1 \\
0
\end{array}\right]+k_{2}\left[\begin{array}{l}
0 \\
0 \\
2
\end{array}\right]+k_{3}\left[\begin{array}{l}
0 \\
0 \\
0
\end{array}\right] \\
& c\left(A^{\top}\right)=k_{1}\left[\begin{array}{l}
1 \\
0 \\
0
\end{array}\right]+k_{2}\left[\begin{array}{l}
0 \\
1 \\
0
\end{array}\right]+k_{3}\left[\begin{array}{l}
0 \\
0 \\
1
\end{array}\right]
\end{aligned}
$$

$$
N\left(A^{\top}\right)=k_{1}\left[\begin{array}{c}
-1 \\
-2 \\
0 \\
1
\end{array}\right]
$$

（c）

$$
[A \mid b] \rightarrow\left[\begin{array}{cc|c}
10 & 20 & 3 \\
0 & 11 & 0 \\
0 \\
0000 & 1 & 0 \\
000 & 0 & 0
\end{array}\right]
$$

特䑲：$x_{r}=\left[\begin{array}{c}1 \\ -1 \\ 0 \\ 0\end{array}\right]$
通解：$x_{p}=k\left[\begin{array}{c}-2 \\ -1 \\ 0\end{array}\right]$

$$
\Rightarrow x=x_{1}+x_{p}=\left[\begin{array}{c}
-1 \\
-1 \\
0
\end{array}\right]+k\left[\begin{array}{c}
-2 \\
-1 \\
0
\end{array}\right]
$$

5．（a）（1）$v_{1}, v_{2}$ 线性无关
Ө $V, \underline{Z} \in \mathrm{~V}$ ，代入
（3） $\operatorname{span}\left(v_{1}, v_{2}\right) \geq V$
解 $\left.x_{1}+x_{2}+k_{3}=v=\right) k_{1}\left[\begin{array}{c}1 \\ 0 \\ 1\end{array}\right]+k_{2}\left[\begin{array}{c}1 \\ -1 \\ 0\end{array}\right]$
（b）$T\left(v_{1}, v_{2}\right)=\left(e_{1}, e_{2}, e_{3}\right) A_{3 x_{2}}$
线生变换： $7 . V^{n} \rightarrow W^{m}$
（国顾）

$$
\begin{aligned}
& T\left(v_{1}\right)=\left[\begin{array}{c}
-3 \\
-1
\end{array}\right]=\left[\begin{array}{lll}
e_{1} & e_{2} & e_{3}
\end{array}\right]\left[\begin{array}{c}
-3 \\
-1
\end{array}\right] \quad v, v_{1} \ldots, v_{n} \rightarrow w_{1}, \ldots, w_{m} \\
& T\left(v_{2}\right)=\left[\begin{array}{c}
-L \\
-1
\end{array}\right]=\left(\begin{array}{lll}
1 & e_{2} e_{s}
\end{array}\right)\left[\begin{array}{c}
-i \\
-1
\end{array}\right] \quad \quad T_{v_{1}}: ? \quad T_{L_{2}}=\text { ? } \\
& A=\left[\begin{array}{cc}
-3 & -2 \\
-1 \\
-1 & -1
\end{array}\right] \\
& T\left(v_{1}, v_{2} \ldots v_{n}\right)=\left(T_{v_{1}}, T_{2} \ldots T_{v_{n}}\right) \\
& =\left[\omega_{1} \cdots \omega_{n}\right] A_{m \times n}
\end{aligned}
$$

$$
\begin{aligned}
& {\left[\begin{array}{cc|c}
-3 & 2 & 3 \\
-1 & -1 & 2 \\
-1 & 1
\end{array}\right] \longrightarrow \cdots \longrightarrow\left[\begin{array}{cc|c}
-3 & 2 & 3 \\
0 & 5 & 3 \\
0 & -5 & 0
\end{array}\right] \text { 呒解 }} \\
& \text { 或 } 7\left(\left[\begin{array}{l}
x_{1} \\
x_{1}
\end{array}\right]\right)=\left[\begin{array}{c}
x_{x_{1}}-x_{2} \\
x_{1}, x_{2} \\
x_{1}
\end{array}\right]:\left[\begin{array}{l}
3 \\
1
\end{array}\right] \text { 求证无解 }
\end{aligned}
$$

C．（a）不始设 $B_{1}, B_{2} \in U$

$$
\begin{gathered}
A B_{1}=B_{1} A, A B_{2}=B_{2} A \\
\Rightarrow A\left(B_{1}+B_{2}\right)=A B_{1}+A B_{2} \quad \text { 验佂加法, 数乘封闭 } \\
A\left(k B_{1}\right)=k\left(A B_{1}\right)
\end{gathered}
$$

（b）$B^{2}\left[\begin{array}{lll}b_{11} & b_{21} & b_{13} \\ b_{1} & b_{2} & b_{23} \\ b_{31} & b_{32} & b_{33}\end{array}\right]$

$$
\begin{gathered}
A B=\left[\begin{array}{ccc}
b_{11}+b_{21}+b_{31} & b_{12}+b_{31}+b_{32} & b_{13}+b_{12}+b_{33} \\
b_{37} & -b_{32} & b_{33} \\
-b_{31} & -b_{32} & -b_{33}
\end{array}\right] \\
B A=\left[\begin{array}{lll}
b_{11} & b_{11} & b_{11}+b_{12}-b_{13} \\
b_{21} & b_{21} & b_{21}+b_{2}-b_{23} \\
b_{31} & b_{31} & b_{33}+b_{32}-b_{33}
\end{array}\right] \\
\Delta \\
A B=13 A \Rightarrow\left(A B B_{1 j}=\left(B A A_{1 j}\right.\right.
\end{gathered}
$$

$$
\begin{gathered}
\Rightarrow b_{31}=0, b_{32}=0, b_{21}=0 \\
b_{22}-b_{23}=b_{33} \quad v \\
b_{11}=b_{12}+b_{22} \quad v \\
b_{11}+b_{12}-b_{13}=b_{13}+b_{23}+b_{33} \Rightarrow b_{12}=b_{33} \\
B=\left[\begin{array}{ccc}
b_{12}+b_{22} & b_{12} & b_{12} \\
0 & b_{22} & b_{23} \\
0 & 0 & b_{22}-b_{23}
\end{array}\right] \\
\left.b_{213}\right\}:\left\{\left[\begin{array}{lll}
1 & 1 & 1 \\
0 & 0 & 0 \\
0 & 0 & 0
\end{array}\right],\left[\begin{array}{lll}
1 & 0 & 0 \\
0 & 1 & 0 \\
0 & 0 & 1
\end{array}\right],\left[\begin{array}{ccc}
0 & 0 & 0 \\
0 & 0 & 1 \\
0 & 0 & -1
\end{array}\right]\right\}
\end{gathered}
$$

(c) $\operatorname{dim}(u)=3$
7. (a) $\quad C\left(A^{\top}\right): V_{1}, \ldots, V_{s}$
$N(A): w_{1}, \ldots, w_{t}$

结改

$$
C\left(A^{\top}\right) \perp N(A)
$$

$$
\begin{aligned}
& t=R(M(A))=n \cdot R(A)=n-\operatorname{dim}\left(C\left(A^{\top}\right)\right)=n-s \\
& \Rightarrow s+t=n \\
& k_{1} v_{1}+\ldots+k_{s} v_{s}+\cdots+k_{n} w_{t}=0 \quad \Leftrightarrow / k_{i}=0, i=1,2, \ldots, n . \\
& A=\left[\begin{array}{lll}
\alpha_{1} & \alpha & \ldots
\end{array}\right] \quad \alpha_{m}^{\top}=\left[\frac{\alpha_{1}^{\top}}{\frac{\alpha}{\alpha_{m}^{\top}}}\right] \\
& C\left(A^{\top}\right)=\operatorname{spcos}\left(\alpha_{1} \cdots \alpha_{m}\right) \\
& N(A)=\{x: A x=0\} \\
& =\left\{x: \alpha_{i}^{\top} x-0, i=1,2, \ldots, m\right\} \\
& \Leftrightarrow V_{i}^{\top} w_{j}=0, i 21, \cdots, s, j=1, \ldots, t \\
& N(A) \perp C\left(A^{\top}\right)
\end{aligned}
$$

$$
\begin{aligned}
& \alpha=k_{1} v+\cdots+k_{1} v_{s}+\cdots+k_{h} w_{t}=0 \\
& \Rightarrow v+w=v \\
& v^{\top}(v+w)=v^{\top} v=0 \quad \exists v=0 \\
& \Rightarrow k_{1}, \ldots, k_{s}=0 \\
& \text { 同理 } k_{s+1}, \cdots k_{n}=0 . \\
& \Rightarrow \text { 线性无关 } \Rightarrow \text { 为一组基. }
\end{aligned}
$$

（b）$A \in \mathbb{R}^{m \times n}$

$$
\begin{aligned}
& K(A)=m \Rightarrow R\left(A^{\top}\right)=m \\
& K\left(A A^{\top}\right)=m-N\left(A A^{\top}\right)=m-N\left(A^{\top}\right)=m-(m-R(A))=P(A)
\end{aligned}
$$

