# 2023秋线性代数期中-答案

> Suggested solutions. $Nov.^{12} 2023$

## Question 1

(1) $A$

(2) $B$

(3) $D$

(4) $B$

(5) $D$

## Question 2

(1) 21

(2) $-A^{-1} C B^{-1}$

(3) 1 or -3

(4)

$$
\left[
\begin{array}{c}
\frac{19}{11} \\
\frac{-5}{11} \\
\end{array}
\right]
$$

(5)

$$
\pm \frac{1}{\sqrt{6}}
\left[
\begin{array}{l}
1 \\ 2 \\ 1
\end{array}
\right]
$$

## Question 3

(A)

A basis for $C(A)$:

$$
\left\{
\left[
\begin{array}{c}1 \\ 0 \\ -1 \\ 2\end{array}
\right],
\left[
\begin{array}{c}2 \\ 1 \\ 1 \\ 0\end{array}
\right],
\left[
\begin{array}{c}1 \\ 1 \\ 3 \\ 1\end{array}
\right]
\right\}
$$

$A$ basis for $C(A^{\top})$:

$$
\left\{
\left[
\begin{array}{c}1 \\ 0 \\ 1 \\ 0 \\ 3\end{array}
\right],
\left[
\begin{array}{c}0 \\ 1 \\ 2 \\ 0 \\ 1\end{array}
\right],
\left[
\begin{array}{c}0 \\ 0 \\ 0 \\ 1 \\ 1\end{array}
\right]
\right\}
$$

or

$$
\left\{
\left[
\begin{array}{c}1 \\ 2 \\ 5 \\ 1 \\ 6\end{array}
\right],
\left[
\begin{array}{c}0 \\ 1 \\ 2 \\ 1 \\ 2\end{array}
\right],
\left[
\begin{array}{c}-1\\ 1 \\ 1 \\ 3 \\ 1\end{array}
\right]
\right\}
$$

$A$ basis for $N(A)$:

$$\left\{
\left[
\begin{array}{c}-1 \\ -2 \\ 1 \\ 0 \\ 0\end{array}
\right],
\left[
\begin{array}{c}-3 \\ -1 \\ 0 \\ -1 \\ 1\end{array}
\right]
\right\}
$$

A basis for $N(A^{\top}):\left\{\left[
\begin{array}{c}-5 \\ 13 \\ -3 \\ 1\end{array}
\right]\right\}$

(B) $\left[
\begin{array}{l}5 \\ 2 \\ 1 \\ 2\end{array}
\right]$

## Question 4

Gaussian Eliminations give:

$$
\left[
\begin{array}{ccc|cc}
1 & -1 & -1 & 2 & 2 \\
2 & a & 1 & 1 & a \\
-1 & 1 & a & -a-1 & -2
\end{array}
\right]
$$

$$
\rightarrow
\left[
\begin{array}{ccc|cc}
1 & -1 & -1 & 2 & 2 \\
0 & a+2 & 3 & -3 & a-4 \\
0 & 0 & a-1 & 0 & 0
\end{array}
\right]
$$

### case1

If $a=-2$, then $\operatorname{rank} A=2 \neq 3=\operatorname{rank}(A ; B)$

$AX=B$ has no solution

### case2

If $a \neq 1$ and $a \neq-1$, $AX=B$ has a unique solution

$$
\left[
\begin{array}{ccc|c}
1 & -1 & -1 & 2 \\
0 & a+2 & 3 & -3 \\
0 & 0 & a-1 & 1-a
\end{array}
\right]
$$

$$
\Rightarrow x=
\left[
\begin{array}{c}
1 \\
0 \\
-1
\end{array}
\right]
$$

$$
\left[
\begin{array}{ccc|c}
1 & -1 & -1 & 2 \\
0 & a+2 & 3 & a-4 \\
0 & 0 & a-1 & 0
\end{array}
\right]
$$

$$
\Rightarrow x=
\left[
\begin{array}{c}
\frac{3a}{a+2} \\
\frac{a-4}{a+2} \\
0
\end{array}
\right]
$$

$$
X=\left[
\begin{array}{cc}
1 & \frac{3a}{a+2} \\
0 & \frac{a-4}{a+2} \\
-1 & 0
\end{array}
\right]
$$

### case3

If $a=1$, $Ax=B$ has infinitely many solutions

$$
\left[
\begin{array}{ccc|c}
1 & -1 & -1 & 2 \\
0 & 3 & 3 & -3 \\
0 & 0 & 0 & 0
\end{array}
\right]
$$

$$
\Rightarrow
x= \left[
\begin{array}{c}
1 \\
-1 \\
0
\end{array}
\right]
+k_{1}\left[
\begin{array}{c}
0 \\
-1 \\
1
\end{array}
\right]
$$

$$
\left[
\begin{array}{ccc|c}
1 & -1 & -1 & 2 \\
0 & 3 & 3 & -3 \\
0 & 0 & 0 & 0
\end{array}
\right]
$$

$$
\Rightarrow
x = \left[
\begin{array}{c}
1 \\
-1 \\
0
\end{array}
\right]
+k_{2} \left[
\begin{array}{c}
0 \\
-1 \\
1
\end{array}
\right]
$$

$$
\Rightarrow X =
\left[
\begin{array}{cc}
1 & 1 \\
-k_{1}-1 & -k_{2}-1 \\
k_{1} & k_{2}
\end{array}
\right]
, \quad k_{1}, k_{2} \text{ arbitrary constants}
$$

## Question 5

(A) Let $X, Y \in M_{2 \times 2}(\mathbb{R})$ and $c \in \mathbb{R}$, then we have

$$
T(C X+Y)=
\left[
\begin{array}{l}
\operatorname{tr} A^{\top}(C X+Y) \\
\operatorname{tr} B^{\top}(C X+Y) \\
\operatorname{tr} C^{\top}(C X+Y)
\end{array}
\right] \\
=C\left[
\begin{array}{c}
\operatorname{tr}(A^{\top} X) \\
\operatorname{tr}(B^{\top} X) \\
\operatorname{tr}(C^{\top} X)
\end{array}
\right]
+ \left[
\begin{array}{c}
\operatorname{tr}(A^{\top} X) \\
\operatorname{tr}(B^{\top} Y) \\
\operatorname{tr}(C^{\top} Y)
\end{array}
\right] \\
=C T(X)+T(Y)
$$

(B)

$$
T(v_{1})=\left[
\begin{array}{l}
1 \\
0 \\
0
\end{array}
\right]=1 \cdot
\left[
\begin{array}{l}
1 \\
0 \\
0
\end{array}
\right]+0\left[
\begin{array}{l}
0 \\
1 \\
0
\end{array}
\right]+0\left[
\begin{array}{l}
0 \\
0 \\
0
\end{array}
\right]
$$

$$
T(v_{2})=\left[
\begin{array}{l}
-1 \\
0 \\
0
\end{array}
\right]=-1\left[
\begin{array}{l}
1 \\
0 \\
0
\end{array}
\right]+0\left[
\begin{array}{l}
0 \\
1 \\
0
\end{array}
\right]+0 \cdot
\left[
\begin{array}{l}
0 \\
0 \\
1
\end{array}
\right]
$$

$$
T(v_{3})=
\left[
\begin{array}{l}
0 \\
1 \\
1
\end{array}
\right]=0
\left[
\begin{array}{l}
1 \\
0 \\
0
\end{array}
\right]+1 \cdot
\left[
\begin{array}{l}
0 \\
1 \\
0
\end{array}
\right]+1 \cdot
\left[
\begin{array}{l}
0 \\
0 \\
1
\end{array}
\right]
$$

$$
T(v_{4})=
\left[
\begin{array}{l}
0 \\
1 \\
-1
\end{array}
\right]=0
\left[
\begin{array}{l}
1 \\
0 \\
0
\end{array}
\right]+1 \cdot
\left[
\begin{array}{l}
0 \\
1 \\
0
\end{array}
\right]+-1 \cdot
\left[
\begin{array}{l}
0 \\
0 \\
1
\end{array}
\right]
$$

Therefore, the matrix representation of $T$ with respect to $v_{1}, v_{2}, v_{3}, v_{4}$ and $w_{1}, w_{2}, w_{3}$ is:

$$
\left[
\begin{array}{cccc}
1 & -1 & 0 & 0 \\
0 & 0 & 1 & 1 \\
0 & 0 & 1 & -1
\end{array}
\right]
$$

(C) Since

$$
T(A)=\left[
\begin{array}{l}
2 \\ 0 \\ 0
\end{array}
\right], T(B)=
\left[
\begin{array}{l}
0 \\ 1 \\ 0
\end{array}
\right], T(C)=
\left[
\begin{array}{l}
0 \\ 0 \\ 1
\end{array}
\right]
$$

we can take $X$ to be

$$
\frac{1}{2} A-2 B+C \\
= \left[
\begin{array}{cc}
\frac{1}{2} & 0 \\
0 & \frac{-1}{2}
\end{array}
\right]-
\left[
\begin{array}{ll}
0 & 2 \\
0 & 0
\end{array}
\right]+
\left[
\begin{array}{ll}
0 & 0 \\
1 & 0
\end{array}
\right]  \\
= \left[
\begin{array}{cc}
\frac{1}{2} & -2 \\
1 & \frac{-1}{2}
\end{array}
\right]
$$

## Question 6

Apply Elementary Row and Column operations to $A$ and $C$ obtain

$$
D_{1}=\left[
\begin{array}{cc}
I_{r} & 0 \\
0 & 0
\end{array}
\right] \text { for } A \text { and } D_{2}=\left[
\begin{array}{cc}
I_{s} & 0 \\
0 & 0
\end{array}
\right]  \text { for } C
$$

Where $r=\operatorname{rank} A, s=\operatorname{rank} C$

Let M=

$$
\left[
\begin{array}{ll}
A & B \\
0 & C
\end{array}
\right]
$$

Then $M$ can be converted to

$$
M_{1}=\left[
\begin{array}{ll}
D_{1} & C_{1} \\
0 & D_{2}
\end{array}
\right]
$$

via elementary row and column operations

Furthermore, the pivots in $D_{1}$ and $D_{2}$ can be used to eliminate the nonzero entries in $C_{1}$, to obtain

$$
M_{2}=\left[
\begin{array}{cccc}
I_{r} & 0 & 0 & 0 \\
0 & 0 & 0 & C_{2} \\
0 & 0 & I_{s} & 0 \\
0 & 0 & 0 & 0
\end{array}
\right]
$$

In conclusion,

$$
\operatorname{rank} M=\operatorname{rank} M_{1}=\operatorname{rank} M_{2}=r+s+\operatorname{rank} C_{2} \geq r+s \\
=\operatorname{rank} A+\operatorname{rank} C \\
$$
