$\underline{\quad\quad\quad}$

（2020-2021期中高数上

I．（1）B

（ $f(x)=|x| \sin x=\left\{\begin{array}{ll}x \sin x, & x \geqslant 0 \\ -x \sin x, & x<0\end{array} \quad f^{\prime}(x)=\left\{\begin{array}{l}\sin x+x \cos x, x \geqslant 0 \\ -\sin x \times \cos x, x<0\end{array}\right.\right.$

$$
f^{\prime}(0)=\lim\limits_{x \rightarrow 0} \frac{f(x)-f(0)}{x}=\lim\limits_{x \rightarrow 0} \frac{|x|}{x} \sin x=0
$$

$\Rightarrow f_{+}^{\prime \prime}(0)=\lim\limits_{x \rightarrow 0^{+}} \frac{f^{\prime}(x)-f^{\prime}(0)}{x}=\lim\limits_{x \rightarrow 0} \frac{\sin x+x \cos x}{x}=\lim\limits_{x \rightarrow 0}\left(\frac{\sin x}{x}+\cos x\right)=2$

ล $f(0)=\lim\limits_{x \rightarrow 0^{-}}\left(-\frac{\sin x}{x}-\cos x\right)=-2$

$\rightarrow f^{(2)}(0)$ does not exist．

$\Rightarrow f^{(n)}(0)$ exists，$n$ 最大是 $n=1$

$$
\begin{aligned}
& \text { (2) A. } \\
& \lim\limits_{x \rightarrow \infty}\left(\frac{x^{2}+1}{x+1}-a x-b\right)=\frac{1}{2} \Rightarrow \text { 户े } \text { i土 }^{y=a x+b+\frac{1}{2}} \quad y=\frac{x^{2}+1}{x+1}=x-1+\frac{2}{x+1} \\
& \text { 的: 斩近线 } \Rightarrow a x+b+\frac{1}{2}=x-1 \\
& \therefore\left\{\begin{array} { l }
{ a = 1 } \\
{ b + \frac { 1 } { 2 } = - 1 }
\end{array} \Rightarrow \left\{\begin{array}{l}
a=1 \\
b=-\frac{3}{2}
\end{array}\right.\right. \\
& \text { 忶 }=: a=\lim\limits_{x \rightarrow \infty} \frac{\frac{x^{2}+1}{x+1}}{x}=1 \\
& b=\lim\limits_{x \rightarrow \infty}\left(\frac{x^{2}+1}{x+1}-x-\frac{1}{2}\right)=\lim\limits_{x \rightarrow \infty}\left(\frac{1-x}{x+1}-\frac{1}{2}\right)=-1-\frac{1}{2}=-\frac{3}{2} \text {. }
\end{aligned}
$$

$\underline{\quad\quad\quad}$

13) B

$$
g(c)=\frac{\int_{0}^{6}\left(x^{2}+6\right) d x}{6}=\frac{\left.\frac{1}{3} x^{3}+6 x\right]_{0}^{6}}{6}=\frac{1}{3} \times 36+6=18
$$

(4). $D$

c). $f(x)=|x| \sin (x) \Rightarrow f^{\prime}(0)=\lim\limits_{x \rightarrow 0} \frac{f(x)-f(0)}{x}=\lim\limits_{x \rightarrow 0} \frac{|x|}{x} \sin |x|=0$.

$$
f(x)=|x| \sin \sqrt{|x|} \rightarrow f^{\prime}(0)=\lim\limits_{x \rightarrow 0} \frac{f(x)-f(0)}{x}=\lim\limits_{x \rightarrow 0} \frac{|x|}{x} \sin \sqrt{|x|}=0 .
$$

$$
f(x)=\cos |x| \quad \rightarrow f^{\prime}(0)=\lim\limits_{x \rightarrow 0} \frac{f(x)-f(0)}{x}=\lim\limits_{x \rightarrow 0} \frac{\cos |x|-1}{x}=\lim\limits_{x \rightarrow 0} \frac{\sin ^{2}|x|}{x} \cdot \frac{1}{\cos |x|+1}
$$

$$
=\frac{-1}{2} \lim\limits_{x \rightarrow 0}\left(\frac{\sin |x|}{|x|}\right)^{2} \frac{|x|^{2}}{x \rightarrow 0}=0 .
$$

$$
\begin{aligned}
f(x)=\cos \sqrt{|x|} \Rightarrow f^{\prime}(0) & =\lim\limits_{x \rightarrow 0} \frac{f(x)-f(0)}{x}=\lim\limits_{x \rightarrow 0} \frac{\cos \sqrt{x \mid}-1}{x}=\lim\limits_{x \rightarrow 0} \frac{-\sin ^{2} \sqrt{|x|}}{x} \\
& =\frac{-1}{2} \lim\limits_{x \rightarrow 0}\left(\frac{\sin \sqrt{|x|}}{\sqrt{|x|}}\right)^{2} \cdot \frac{|x|}{x}=\left\{\begin{array}{l}
\frac{1}{2}=f^{\prime}(0) \\
\frac{1}{2}=f^{\prime}(0)
\end{array}\right.
\end{aligned}
$$

$\Rightarrow f^{\prime}(0)$ does not expst.

(5) C

$$
\begin{aligned}
f(x)=\frac{1-\sin x}{1+\sin x} \Rightarrow f^{\prime}(x) & =\frac{-\cos x(1+\sin x)-\cos x(1-\sin x)}{(1+\sin x)^{2}}=\frac{-2 \cos x}{(1+\sin x)^{2}} \\
f^{\prime}\left(\frac{\pi}{6}\right) & =\frac{-2 x \frac{\sqrt{3}}{2}}{\left(\frac{3}{2}\right)^{2}}=-\frac{4 \sqrt{3}}{9}=-\frac{4}{3 \sqrt{3}}
\end{aligned}
$$

2(1) $0 . \quad \int_{-2}^{\frac{\pi}{2}} \frac{\sin ^{5} x \cos ^{3} x}{\text { 大数 }} d x=0$

(2) $\frac{1}{1^{2}} \cdot \int_{0}^{x^{3}-1} f(t) d t=x \Rightarrow 3 x^{2} f\left(x^{3}-1\right)=1$ (et $x=2 \Rightarrow f(7)=\frac{1}{12}$

(3) $\frac{1}{3} x^{3}+2 x-\frac{1}{x}-\frac{4}{3}, \quad f^{\prime}(x)=\left(x+\frac{1}{x}\right)^{2}=x^{2}+2+\frac{1}{x^{2}}$

$$
\Rightarrow f(x)=\frac{1}{3} x^{3}+2 x-\frac{1}{x}+c, f(1)=1 \Rightarrow c=-\frac{4}{3}
$$

(4) $-2, \quad x^{2}+y^{2}+z^{2}=13^{2} \Rightarrow 2 x \cdot x^{\prime}+2 y \cdot y^{\prime}+2 z \cdot z^{\prime}=0$.

let $t=x_{0} . x\left(t_{0}\right)=3, x^{\prime}\left(t_{0}\right)=4, y\left(t_{0}\right)=4, y^{\prime}\left(t_{0}\right)=3$

$$
z\left(t_{0}\right)=12
$$

$$
\Rightarrow 24+24+24 z^{\prime}\left(t_{0}\right)=0 \Rightarrow z^{\prime}\left(t_{0}\right)=-2 .
$$

5. $\frac{a}{\sqrt{a^{2}+1}} \cdot \lim\limits_{s \rightarrow a} \frac{\sqrt{s^{2}+1}-\sqrt{a^{2}+1}}{s-a}=\left.\frac{d}{d s}\left(\sqrt{s^{2}+1}\right)\right|_{s=a}=\frac{a}{\sqrt{a^{2}+1}}$

3. (1) $\lim\limits_{x \rightarrow \infty} \frac{\sqrt{3+x}-\sqrt{x+1}}{x^{2}+x-2}=\lim\limits_{x \rightarrow \infty} \frac{\frac{\sqrt{3+x}}{x^{2}}-\frac{\sqrt{x+1}}{x^{2}}}{1+\frac{1}{x}-\frac{2}{x^{2}}}=0$

12) $\left.\lim\limits_{x \rightarrow 0} \frac{\cos x-\sec ^{2} x}{x \sin x}=\lim\limits_{x \rightarrow 0} \frac{\cos x-\frac{1}{\cos ^{2} x}}{x \sin x}=\lim\limits_{x \rightarrow 0} \frac{\cos ^{3} x-1}{x \sin x}=\lim\limits_{x \rightarrow 0} \frac{(\cos x-1)}{x \sin x} \cdot \cos ^{2} x+\cos x+1\right)$

$=3 \lim\limits_{x \rightarrow 0} \frac{\cos x-1}{x \sin x}=3 \lim\limits_{x \rightarrow 0} \frac{-\sin ^{2} x}{x \sin x} \cdot \frac{1}{\cos x+1}=\frac{3}{-2} \lim\limits_{x \rightarrow 0} \frac{\sin x}{x}=-\frac{3}{2}$

4. (1) $\left.\int_{0}^{2 \pi}\left|\sin ^{2} x-\cos ^{2} x\right| d x=\int_{0}^{2 \pi}|\cos 2 x| d x=8 \int_{0}^{\frac{2}{4}} \cos 2 x d x=4 \sin 2 x\right]_{0}^{\frac{2}{4}}=4$.

![](https://cdn.mathpix.com/cropped/2025_04_21_0457eb8051300bf4b199g-3.jpg?height=164&width=678&top_left_y=1997&top_left_x=569)

12) $\int_{0}^{1}(x+2) \sqrt{1-x^{2}} d x=\int_{0}^{1} x \sqrt{1-x^{2}} d x+2 \int_{0}^{1} \sqrt{1-x^{2}} d x=-\frac{1}{3}\left(1-x^{2}\right)^{\frac{3}{2}} \int_{0}^{1}+2 x \frac{x}{4}=\frac{1}{3}+\frac{\pi}{2}=$

5. $f(x)=\frac{x^{3}+x-2}{x-x^{2}}$

(i) $f(x)=\frac{x^{3}+x-2}{x-x^{2}}=\frac{(x-1)\left(x^{2}+x+2\right)}{x(1-x)}=\frac{x^{2}+x+2}{x}=-x-1-\frac{2}{x} \quad$ domain. $x \neq 0$. $x=1$.

$f^{\prime}(x)=-1+\frac{2}{x^{2}}, \quad f^{\prime \prime}(x)=-\frac{4}{x^{3}}$

let $f^{\prime}(x)=0 \Rightarrow x= \pm \sqrt{2} \quad x^{-1} x-\sqrt{2} \Rightarrow f^{\prime}(x)<0 \downarrow \quad f(\sqrt{2})=-\sqrt{2}+-\frac{2}{\sqrt{2}}=-2 \sqrt{2}-1$

citifical points at $x= \pm \sqrt{2}$

![](https://cdn.mathpix.com/cropped/2025_04_21_0457eb8051300bf4b199g-4.jpg?height=275&width=912&top_left_y=1079&top_left_x=772)

$f^{\prime \prime}(x)=\frac{4}{-x^{3}} \Rightarrow x<0, f^{\prime \prime}(x)>0$ concave up but $x \neq 0 \Rightarrow$ hes inflection print $x>0, f^{\prime}(x)<0$ concave down.

(2) horizontal agunptote: no. vertical asymptote: $x=0$. oblique asymptote: $\quad y=-x-1$

![](https://cdn.mathpix.com/cropped/2025_04_21_0457eb8051300bf4b199g-4.jpg?height=603&width=660&top_left_y=1589&top_left_x=915)

$\underline{\quad\quad\quad}$

$\underline{\quad\quad\quad}$

$\underline{\quad\quad\quad}$

6. (1) $y=\int_{1}^{1+2 x} \sqrt{t^{2}-1} d t \rightarrow \frac{d y}{d x}=2 \sqrt{(1+2 x)^{2}-1}=2 \sqrt{4 x^{2}+4 x}$

(2) $x^{2}-y^{2}=9 \Rightarrow 2 x-2 y \cdot \frac{d y}{d x}=0 \Rightarrow \frac{d y}{d x}=\frac{x}{y}=-\frac{5}{4}$.

$$
y-(-4)=-\frac{5}{4}(x-5)
$$

T. $\left\{\begin{array}{l}y=x^{2} \\ y=2 x-x^{2}\end{array} \Rightarrow 2 x^{2}=2 x \Rightarrow x=0, x=1\right.$.

![](https://cdn.mathpix.com/cropped/2025_04_21_0457eb8051300bf4b199g-5.jpg?height=212&width=452&top_left_y=842&top_left_x=1282)

$\left.s=\int_{0}^{1}\left[\left(2 x-x^{2}\right)-x^{2}\right] d x=\int_{0}^{1}\left(2 x-2 x^{2}\right) d x=x^{2}-\frac{2}{3} x^{3}\right]_{0}^{11}=1-\frac{2}{3}=\frac{1}{3}$

$$
\text { 8. } \begin{aligned}
& \begin{array}{l}
y=\sqrt{x} \\
y=2 x-1
\end{array} \Rightarrow x^{2}=4 x^{2}-4 x+1(3 x-1)(x-1)=0 \\
& 3 x^{2}-4 x+1=0 \quad x=\frac{1}{3}, x=1
\end{aligned}, ~ \begin{aligned}
V & =2 \pi \int_{0}^{1}(x+1)(\sqrt{x}-(2 x-1)) d x \\
& =2 \pi \int_{0}^{1}\left(x^{\frac{3}{2}}-2 x^{2}+x+\sqrt{x}-2 x+1\right) d x \\
& \left.=2 \pi\left(\frac{2}{5} x^{\frac{5}{2}}-\frac{2}{3} x^{3}-\frac{1}{2} x^{2}+\frac{2}{3} x^{\frac{3}{2}}+x\right)\right]_{0}^{1} \\
& =2 \pi\left(\frac{2}{5}-\frac{2}{3}-\frac{1}{2}+\frac{2}{3}+1\right)=\frac{9 \pi}{5} .
\end{aligned}
$$

![](https://cdn.mathpix.com/cropped/2025_04_21_0457eb8051300bf4b199g-5.jpg?height=313&width=355&top_left_y=1237&top_left_x=1282)

9. $f(x)$ is continuous on 6,1$] \Rightarrow f(x)$ has max, min., $f(\alpha)=M=f(x)$.

$$
f(\beta) \leqslant \int_{e}^{1} f(x) d x \leqslant f(\alpha)
$$

