# 2018 期中

## 1 选择题

### 1-1
B

### 1-2
C

### 1-3
$P(X \geq 1) =1-P(X<1) =1-P(X=0) =1-(1-p)^{2}=\frac{5}{9} \Rightarrow 1-p=\frac{2}{3} \Rightarrow p=\frac{1}{3}$,

$P(Y=1) =1-P(Y=0) =1-\left(\frac{2}{3}\right)^{3}=\frac{19}{27} \quad B$

### 1-4
$P_{1}=P(-2<X<2) \quad P_{2}=P(-1<X<1) \quad P_{3}=P\left(-\frac{1}{3}<X<-1\right)$

$P_{1}>P_{2}>P_{3} \quad A$

### 1-5
C

## 2 填空题

### 2-1
$2 \cdot \frac{1}{120}=\frac{1}{60}$

### 2-2
$0.4 \times 0.3 \times 0.5+0.6 \times 0.3 \times 0.5+0.4 \times 0.7 \times 0.5=0.29$

$P(X \mid B) =0.4 \times 0.5+0.6 \times 0.5=0.5$

$P(X \mid B) \cdot P(B) =P(B \mid X) \cdot P(X) \Rightarrow P(B \mid X) =\frac{P(X \mid B) \cdot P(B)}{P(X)}=\frac{0.5 \times 0.3}{0.29}=\frac{15}{29}$

### 2-3
$P_{1}=(0.6) ^{3} \quad P_{2}=(0.4) ^{3} \quad P=1-P_{1}-P_{2}=0.72$

### 2-4
$P(\bar{A} \cup \bar{B}) =1-P(A \cap B) =1-[P(A \cup B) -P(A) -P(B)]=1-\left(\frac{4}{3}-1\right) =\frac{2}{3}$

### 2-5
$f(x) =\left\{\begin{array}{cc}\lambda e^{-\lambda x} & x \geq 0 \\ 0 & x<0\end{array}\right.$

$P(3<X<4) =\int_{3}^{4} \lambda e^{-\lambda x} dx=e^{-3 \lambda}-e^{-4 \lambda} \quad P(X>2) =\int_{2}^{\infty} \lambda e^{-\lambda x} dx=e^{-2 \lambda}$

$P(3<X<4 \mid X>2) =e^{-\lambda}-e^{-2 \lambda}=t-t^{2}=-\left(t-\frac{1}{2}\right)^{2}+\frac{1}{4} \quad t=e^{-\lambda}=\frac{1}{2} \Rightarrow \lambda=\ln 2$

### 2-6
$P(\max (X, Y) >2) =1-P(\max (X, Y) \leq 2) =1-P(X \leq 2, Y \leq 2) =1-P(X \leq 2) P(Y \leq 2)$

$=1-\frac{1}{2} \cdot \frac{1}{2}=\frac{3}{4}$

### 2-7
$X-Y \sim N(-\mu, 2\sigma^{2}) \quad -\mu=2 \Rightarrow \mu=-2$

### 2-8
$P(X=k) =\frac{\lambda^{k}}{k!} e^{-\lambda}$

$$
P(Y=k) =P\left(X=k^{1/3}\right) =\frac{\lambda^{k^{1/3}}}{(k^{1/3})!} e^{-\lambda}
$$

## 3 解答题

### 3-1

$P=P(X \leq 2/3) =\int_{0}^{2/3} 3x^{2} dx=\left(\frac{2}{3}\right)^{3}=\frac{8}{27}$

$P(i=1) =\binom{3}{1} \cdot P \cdot (1-P)^{2}=3 \cdot \frac{8}{27} \cdot\left(1-\frac{8}{27}\right)^{2}=\frac{2888}{6561}$

### 3-2

(1) $\frac{1}{6}+a+\frac{1}{18}+\frac{1}{3}+\frac{2}{9}+b=\frac{7}{9}+a+b=1 \Rightarrow a+b=\frac{2}{9}$

(2) $P(X=1) =\frac{1}{2} \quad P(Y=0) =\frac{2}{9}+a$

$P(X=1, Y=0) =\frac{1}{2}\left(\frac{2}{9}+a\right) =\frac{1}{6} \Rightarrow \frac{2}{9}+a=\frac{1}{3} \Rightarrow a=\frac{1}{9} \quad b=\frac{1}{9}$

### 3-3

(1) $\int_{-1}^{1} \int_{x^{2}}^{1} cx^{2}y \, dy \, dx=\int_{-1}^{1} \frac{c}{2}x^{2}(1-x^{4}) \, dx=\frac{4c}{21}=1 \Rightarrow c=\frac{21}{4}$

(2) $\int_{0}^{1} \int_{x^{2}}^{x} cx^{2}y \, dy \, dx=\int_{0}^{1} \frac{c}{2}x^{2}(x^{2}-x^{4}) \, dx=\frac{c}{10}-\frac{c}{14}=\frac{3c}{70}$

### 3-4

$P(X>x) =1-P(X \leq x) \leq 0.05 \Rightarrow P(X \leq x) \geq 0.95 \Rightarrow P\left(\frac{X-110}{12} \leq \frac{x-110}{12}\right) \geq 0.95$

$\Rightarrow \Phi\left(\frac{x-110}{12}\right) \geq 0.95 \Rightarrow \frac{x-110}{12} \geq 1.645 \Rightarrow x \geq 129.74$ 故最小为 129.74

### 3-5

(1) $f(x, y) =\left\{\begin{array}{cc}c & (x, y) \in G \\ 0 & \text{其它}\end{array}\right. \Rightarrow \iint_{(x, y) \in G} f(x, y) \, dx \, dy=c \cdot \frac{1}{2} \cdot 2 \cdot 1=c=1$

$$
f_{X}(x) = \begin{cases}\int_{0}^{x} f(x, y) \, dy=x & 0 \leq x < 1 \\ \int_{0}^{2-x} f(x, y) \, dy=2-x & 1 \leq x \leq 2 \end{cases}
$$

(2) $f_{Y}(y) =\int_{y}^{2-y} f(x, y) \, dx=2(1-y) \quad 0 \leq y \leq 1$

故当 $0 \leq y < 1$ 时，$f_{X \mid Y}(x \mid y) =\frac{f(x, y)}{f_{Y}(y)}=\frac{1}{2(1-y)} \quad y \leq x \leq 2-y$

### 3-6

(1) $P(Y \leq 1) =P\left(Y^{\prime}=1\right) =P(X \equiv 2) =\int_{2}^{3} \frac{1}{9} x^{2} d x=\frac{19}{27}$

$P(i \leq x) =P(Y \leq 1) +P(1<Y<x) =\frac{19}{27}+\int_{1}^{x} \frac{1}{9} t^{2} d t=\frac{19}{27}+\frac{1}{27}\left(x^{3}-1\right) =\frac{1}{27} x^{3}+\frac{2}{3}$

${ }^{y_{22}} P(Y \leq y) =\frac{26}{27}+P(X \leq 1) =1$

故

$$
F_{1}(y) =\left\{\begin{array}{cc}
0 & y<1 \\
\frac{2}{3}+\frac{1}{27} y^{3} & 1 \leqslant y<2 \\
1 & 2 \leqslant y
\end{array}\right
$$

(2) $P\{X \leq Y\}=P(Y=2) +P(Y=X) =P(X<2) =\int_{0}^{2} \frac{1}{9} x^{2} d x=\frac{8}{27}$
