# 2023 Fall Final Exam Solution Set

> Jan 12, 2024

## Choice Answer $15^{\prime}$

+ 1 $D$
+ 2 $C$
+ 3 $B$
+ 4 $B$
+ 5 $A$

## 2  $25^{\prime}$

### (1)

$u^{\top} u+1, 1 ; 1, n-1$ ．

### (2)

$\sqrt{5}, \sqrt{7}$

### (3)

$\left[\begin{array}{ccccc}
0 & 0 & 0 & 0 & 0\\
0 & 0 & 0 & 0 & 0\\
0 & 0 & 1 & 2024 & 1012 \times 2023\\
0 & 0 & 0 & 1 & 2024\\
0 & 0 & 0 & 0 & 1
\end{array}\right]$

### (4)

$\frac{1}{2 \sqrt{2}}\left[(1+\sqrt{2})^{100}-(1-\sqrt{2})^{100}\right]$

### (5)

1,0

## Question 3： $12^{\prime}$

### (a)

There are two eigenvalues of $A: \lambda_{1}=0$ \＆$\lambda_{2}=1$

$A$ basis for the eigen spacer $N(A)$ corresponding to $\lambda_{1}=0$ is：

$$
\left[\begin{array}{c}
-1 \\
-1 \\
1 \\
0 \\
0
\end{array}\right],
\left[\begin{array}{c}
3 \\
-2 \\
0 \\
1 \\
0
\end{array}\right],
\left[\begin{array}{c}
7 \\
-3 \\
0 \\
0 \\
1
\end{array}\right]
$$

A basis for the eigenspace，$N(A-I)$ ，Corresponding to $\lambda_{2}=1$ is：

$$
\left[\begin{array}{c}
1 \\
1 \\
-1 \\
1 \\
0
\end{array}\right],
\left[\begin{array}{l}
3 \\
0 \\
0 \\
0 \\
1
\end{array}\right]
$$

Therefore，

$$
S=\left[\begin{array}{ccccc}
-1 & 3 & 7 & 1 & 3 \\
-1 & -2 & -3 & 1 & 0 \\
1 & 0 & 0 & -1 & 0 \\
0 & 1 & 0 & 1 & 0 \\
0 & 0 & 1 & 0 & 1
\end{array}\right]
$$

### (b)

Since $\quad S^{-1} A S=\Lambda$=$\left[\begin{array}{lllll}
0 & 0 & 0 & 0 & 0 \\
0 & 0 & 0 & 0 & 0 \\
0 & 0 & 0 & 0 & 0 \\
0 & 0 & 0 & 1 & 0 \\
0 & 0 & 0 & 0 & 1 \\
\end{array}\right]$ ，

$$
\begin{aligned}
A=S \Lambda S^{-1} \Rightarrow A^{k} & =S \Lambda^{k} S^{-1} \\
& =S \Lambda S^{-1}=A .
\end{aligned}
$$

## Question 4： $8^{\prime}$

Orthonormalize the columns of $A$ by Gram－Schmidt to obtain

$$
Q=\left[\begin{array}{ccc}
\frac{1}{\sqrt{2}} & \frac{1}{\sqrt{6}} & -\frac{1}{\sqrt{3}} \\
\frac{1}{\sqrt{2}} & -\frac{1}{\sqrt{6}} & \frac{1}{\sqrt{3}} \\
0 & \frac{2}{\sqrt{6}} & \frac{1}{\sqrt{3}}
\end{array}\right]
$$

## Question 5： $20^{\prime}$

### 5-(a)

$
A^{H}=\left[\begin{array}{ccc}
0 & -i & 0 \\
i & 1 & i \\
0 & -i & 0\end{array}\right]^{H}=
\left[\begin{array}{ccc}
0 & -i & 0 \\
i & 1 & i \\
0 & -i & 0\end{array}\right]=A \Rightarrow A
$ is Hermition．

### 5-(b)

$$
\begin{aligned}
& |A-\lambda I|=\left|\begin{array}{ccc}
0-\lambda & -i & 0 \\
i & 1-\lambda & i \\
0 & -i & 0-\lambda
\end{array}\right|=
(-\lambda)(-1)^{1+1}\left[(1-\lambda)(-\lambda)+i^{2}\right] \\
& +(-i)(-1)^{1+2}[(-\lambda) i] \\
& \Rightarrow -\lambda\left(\lambda^{2}-\lambda-1\right)+\lambda=
-\lambda\left(\lambda^{2}-\lambda-2\right)=0 \\
& \Rightarrow \lambda=0,-1,2 .
\end{aligned}
$$

$$
\begin{array}{ll}
\lambda=0:(A-\lambda I) x=0 & \Rightarrow x=\left[\begin{array}{c}
1 \\
0 \\
-1
\end{array}\right] \\
\lambda=-1:(A-\lambda I) x=0 \quad & \Rightarrow x=\left[\begin{array}{c}
1 \\
-i \\
1
\end{array}\right] \\
\lambda=2:(A-\lambda I) x=0 \Rightarrow x=\left[\begin{array}{c}
1 \\
2 i \\
1
\end{array}\right]
\end{array}
$$

### 5-(C)

$$
U=\left[\begin{array}{ccc}
\frac{1}{\sqrt{2}} & \frac{1}{\sqrt{3}} & \frac{1}{\sqrt{6}} \\
0 & -\frac{i}{\sqrt{3}} & 2 i / \sqrt{6} \\
-\frac{1}{\sqrt{2}} & \frac{1}{\sqrt{3}} & \frac{1}{\sqrt{6}}
\end{array}\right] .
$$

## Question 6: $10^{\prime}$

### 6-(a)

$A=\left[\begin{array}{ccc}\lambda-3 & 2 & 0 \\ 2 & \lambda & 0 \\ 0 & 0 & \lambda-1\end{array}\right]$.

$$
\begin{aligned}
& (\lambda-4)(\lambda+1)>0 \\
& (\lambda-1)(\lambda-4)(\lambda+1)<0
\end{aligned}
$$

### 6-(b)

(b) $A$ is negativedefinite if and only if

$$
\begin{aligned}
& \text { 1) } \operatorname{det} A_{1}=\lambda-3<0 \\
& \text { 2) } \operatorname{det} A_{2}=\lambda^{2}-3 \lambda-4>0 \\
& \text { 3) } \operatorname{det} A_{3}=(\lambda-1)\left(\lambda^{2}-3 \lambda-4\right)<0 \\
& \left.\begin{array}{l}
\lambda-4>0 \text { or } \lambda<-1 \\
\lambda-3<0 \\
\lambda-1<0
\end{array}\right\} \Rightarrow \lambda < 1
\end{aligned}
$$

## Question 7

### 7- (a)

Since $A$ has $n$ distinct eigenvalues，$A$ is diagonalizable，ie．there exists an invertible $P$ ，such that

$$
P^{-1} A P=\left[\begin{array}{llll}
\lambda_{1} & & & \\
& \lambda_{2} & & \\
& & \ddots & \\
& & & \lambda_{n}
\end{array}\right]
$$

$$
A B=B A \Rightarrow P^{-1} A P P^{-1} B P=P^{-1} A B P=P^{-1} B A P
$$

$$
=P^{-1} B P P^{-1} A P .
$$

Therefore，we can assume $A$ is a diagonal matrix，that is，

$$
A=\left[\begin{array}{llll}
\lambda_{1} & & & \\
& \lambda_{2} & & \\
& & \ddots & \\
& & & \lambda_{n}
\end{array}\right]
$$

$$
AB=\left[\begin{array}{cccc}
\lambda_{1}b_{11} & \lambda_{1}b_{12} & ... & \lambda_{1}b_{1n}  \\
\lambda_{2}b_{12} & \lambda_{2}b_{22} & ... & \lambda_{2}b_{2n}  \\
... & ... & ... & ...  \\
\lambda_{n}b_{1n} & \lambda_{n}b_{n2} & ... & \lambda_{n}b_{nn}  \\
\end{array}\right] =
\left[\begin{array}{cccc}
\lambda_{1}b_{11} & \lambda_{2}b_{12} & ... & \lambda_{n}b_{1n}  \\
\lambda_{1}b_{21} & \lambda_{2}b_{22} & ... & \lambda_{n}b_{2n}  \\
... & ... & ... & ...  \\
\lambda_{1}b_{n1} & \lambda_{2}b_{n2} & ... & \lambda_{n}b_{nn}  \\
\end{array}\right]
$$

Comparing the entries，we see that $\lambda_{i} b_{i j}=\lambda_{j} b_{i j}, \lambda_{i} \neq \lambda_{j}$ ，$(i \neq j$ hence $b_{i j}=0(i \neq j)$ ．It follows that $B$ is a diagonal matrix．

### 7-(b)

${ }^{(c)} A$ and $B$ can be diagonalized by some invertible matrix $P$ ，icc

$$
P^{-1} A P=\left[\begin{array}{llll}
\lambda_{1} & & & \\
& \lambda_{2} & & \\
& & \ddots & \\
& & & \lambda_{n}
\end{array}\right], \quad P^{-1} B P=\left[\begin{array}{lll}
\mu_{1} & & & \\
& \mu_{2} & & \\
& & \ddots & \\
& & & \mu_{n}
\end{array}\right]
$$

Where $\lambda_{i}, \mu_{i}$ are the eigenvalues of $A$ and $B$ Correspondingly．

Choose $n$ polynomials as follows，

$$
f_{i}(x)=\frac{\left(x-\lambda_{1}\right) \cdots\left(x-\lambda_{i-1}\right)\left(x-\lambda_{i+1}\right) \cdots\left(x-\lambda_{n}\right)}{\left(\lambda_{i}-\lambda_{1}\right) \cdots\left(\lambda_{i}-\lambda_{i-1}\right)\left(\lambda_{i}-\lambda_{i+1}\right) \cdots\left(\lambda_{i}-\lambda_{n}\right)}, \quad i=1,2, \cdots, n
$$

Let $f(x)=\mu_{1} f_{1}(x)+\mu_{2} f_{2}(x)+\cdots+\mu_{n} f_{n}(x)$ ．Then it can be verified that $f\left(\lambda_{i}\right)=\mu_{i}, \quad i=1,2, \cdots, n$ ．

$$
P^{-1} B P=\left[\begin{array}{llll}
f\left(\lambda_{1}\right) & & & \\
& f\left(\lambda_{2}\right) & & \\
& & \ddots & \\
& & & f\left(\lambda_{n}\right)
\end{array}\right]=f\left(P^{-1} A P\right)=P^{-1} f(A) P
$$

thus $\quad B=f(A)$
