# MA127 Calculu II : Midterm I Solution

## 一

### 1-1

$a_{n}=\frac{2^{n}+4^{n}}{3^{n}+4^{n}}=\frac{(\frac{1}{2})^{n}+1}{(\frac{3}{4})^{n}+1} \rightarrow 1$ as $n \rightarrow \infty$

$\therefore a_{n} \not\rightarrow 0 \therefore \sum a_{n}$ div

### 1-2

$f(x)=\frac{1}{x(\ln x)^{2}}, f(x)>0 \& \downarrow$ for $x \geq 2$

$a_{n}=f(n)$ for $n \geq 2$

$$
\int_{2}^{\infty} f(x) d x=
\int_{2}^{\infty} \frac{1}{x(\ln x)^{2}} d x
\overset{u=\ln x, du=\frac{1}{x} dx}{=}
\int_{\ln 2}^{\infty} \frac{1}{u^{2}} d u \quad
\operatorname{conv} . \quad(p=2>1)
$$

$\therefore \sum a_{n}$ conv. \& A.C. $(a_{n}>0)$

### 1-3

$a_{n}=\frac{1}{n \sqrt[n]{n}}, \quad b_{n}=\frac{1}{n}$

$\lim\limits_{n \rightarrow \infty} \frac{a_{n}}{b_{n}}=\lim\limits_{n \rightarrow \infty} \frac{1}{\sqrt[n]{n}}=1 \Rightarrow$ both conv. or both div

$\because \sum b_{n}$ div. $\therefore \Sigma a_{n}$ div

### 1-4

$|\frac{a_{n+1}}{a_{n}}|=\frac{(n+1)!(n+2)!(n+3)!}{(3 n+3)!} \frac{(3 n)!}{n!(n+1)!(n+2)!}=\frac{(n+3)(n+2)(n+1)}{(3 n+3)(3 n+2)(3 n+1)} \rightarrow \frac{1}{27}<1$ as $n \rightarrow \infty$

$\Rightarrow \sum a_{n}$ A.C

### 1-5

$\sum \limits_{n=1}^{\infty}(-1)^{n} u_{n}, u_{n}=\sqrt{n^{2}+1}-n>0$,

$u_{n}=\frac{(\sqrt{n^{2}+1}-n)(\sqrt{n^{2}+1}+n)}{\sqrt{n^{2}+1}+n}=\frac{1}{\sqrt{n^{2}+1}+n}$ down in $n$

$\lim\limits_{n \rightarrow \infty} u_{n}=0$. $\therefore$ it is conv. by alternating series test

$\sum \limits_{n=1}^{\infty} u_{n}=\sum \limits_{n=1}^{\infty} \frac{1}{\sqrt{n^{2}+1}+n}, \quad b_{n}=\frac{1}{n}$

$\frac{u_{n}}{b_{n}}=\frac{n}{\sqrt{n^{2}+1}+n} \rightarrow \frac{1}{2} \quad \therefore \sum u_{n} \& \sum b_{n}$ both conv. or both div.

Since $\sum \frac{1}{n}$ div, $\sum u_{n}$ div. In summary, $\sum(-1)^{n} u_{n}$ is C.C

## 二

### 2-1

$|\frac{a_{n+1}}{a_{n}}|=\frac{|x|^{n+1}}{\sqrt{(n+1)^{2}+3}} \cdot \frac{\sqrt{n^{2}+3}}{|x|^{n}} \rightarrow|x|$

$\therefore$ radius of cone. $r=1$

### 2-2

$x=1$ : $\sum \limits_{n=1}^{\infty}(-1)^{n} \frac{1}{\sqrt{n^{2}+3}}$ conv by alternating series test

$\sum \limits_{n=1}^{\infty} \frac{1}{\sqrt{n^{2}+3}}$ div. since $\frac{\frac{1}{\sqrt{n^{2}+3}}}{\frac{1}{n}} \rightarrow 1 \&  \sum \frac{1}{n}$ div

$\therefore$ C.C. at $x=1$

$x=-1: \sum \limits_{n=1}^{\infty} \frac{1}{\sqrt{n^{2}+3}}$ div

In summary, radius of conv is 1;

interval of conv is $(-1,1]$;

the series is A.C. in $(-1,1)$ \& C.C. at $x=1$

## 三

$$
\begin{aligned}
f(x) & =(x+1) e^{x}=(x+1)[1+x+\frac{x^{2}}{2!}+\frac{x^{3}}{3!}+\cdots] \\
& =1+x+\frac{x^{2}}{2!}+\frac{x^{3}}{3!}+\cdots+x+x^{2}+\frac{x^{3}}{2!}+\frac{x^{4}}{3!}+\cdots \\
& =1+2 x+(\frac{1}{2!}+1) x^{2}+(\frac{1}{3!}+\frac{1}{2!}) x^{3}+\cdots \\
& =1+\sum \limits_{n=1}^{\infty}(\frac{1}{(n-1)!}+\frac{1}{n!}) x^{n}=\sum \limits_{n=0}^{\infty} \frac{n+1}{n!} x^{n}
\end{aligned}
$$

## 四

$\frac{1}{1+x}=\frac{1}{1-(-x)}=1-x+x^{2}-x^{3}+\cdots$

$$
\begin{aligned}
& [\ln (1+x)]^{\prime}=\frac{1}{1+x} \\
\Rightarrow & \ln (1+x)=x-\frac{x^{2}}{2}+\frac{x^{3}}{3}-\frac{x^{4}}{4}+\cdots \\
\Rightarrow & \ln (1+x^{2})=x^{2}-\frac{x^{4}}{2}+\frac{x^{6}}{3}-\frac{x^{8}}{4}+\cdots \\
& \cos x=1-\frac{x^{2}}{2!}+\frac{x^{4}}{4!}-\frac{x^{6}}{6!}+\cdots \\
\Rightarrow & 1-\cos x=\frac{x^{2}}{2!}-\frac{x^{4}}{4!}+\frac{x^{6}}{6!}-\cdots
\end{aligned}
$$

$$
\lim\limits_{x \rightarrow 0} \frac{\ln (1+x^{2})}{1-\cos x}=\lim\limits_{x \rightarrow 0} \frac{x^{2}-\frac{x^{4}}{2}+\frac{x^{6}}{3}-\cdots}{\frac{x^{2}}{2!}-\frac{x^{4}}{4!}+\frac{x^{6}}{6!} \cdots}=2
$$

## 五

$L=\int_{0}^{2 \pi} \sqrt{(\frac{d x}{d t})^{2}+(\frac{d y}{d t})^{2}}=\int_{0}^{2 \pi} \frac{3}{2}|\sin 2 t| d t=(4)(\frac{3}{2}) \int_{0}^{\frac{\pi}{2}} \sin 2 t d t=\left.-3 \cos 2 t\right]_{0}^{\frac{\pi}{2}}=6$

## 六

$r=2 \sin \theta, \frac{\pi}{4} \leqslant \theta \leqslant \frac{\pi}{2}$

$r^{2}=2 r \sin \theta, \quad x^{2}+y^{2}=2 y, \quad x^{2}+(y-1)^{2}=1$

$$
\begin{aligned}
A & =\frac{1}{2} \int_{\frac{\pi}{4}}^{\frac{\pi}{2}} r^{2} d \theta=\int_{\frac{\pi}{4}}^{\frac{\pi}{2}} 2 \sin ^{2} \theta d \theta \\
& =\int_{\frac{\pi}{4}}^{\frac{\pi}{2}}[1-\cos 2 \theta] d \theta=[\theta-\frac{\sin 2 \theta}{2}]_{\frac{\pi}{4}}^{\frac{\pi}{2}}=\frac{\pi}{4}+\frac{1}{2}
\end{aligned}
$$

Alternative method:

$$
\begin{aligned}
A & =\frac{1}{4}(\text { area of disc })+\text { area of the triangle } \\
& =\frac{\pi}{4}+\frac{1}{2}
\end{aligned}
$$

## 七

$(1+x)^{m}=1+\sum \limits_{k=1}^{\infty}\binom{m}{k} x^{k}, \quad(\frac{m}{k})=\frac{m(m-1)(m-2) \cdots(m-k+1)}{k!}$, for $|x|<1$

$(1+x)^{\frac{1}{2}}=1+\frac{1}{2} x-\frac{1}{8} x^{2}+\frac{1}{16} x^{3}+\cdots$ for $|x|<1$

## 八

First assume $\{x_{n}\}$ conv to L

Then $\lim\limits_{n \rightarrow \infty} x_{n+1}=\lim\limits_{n \rightarrow \infty} x_{n}=L$

Thus $L=\frac{L}{2}+\frac{1}{L} \Rightarrow L=\sqrt{2} \quad$ (we observe $L \geq 0$ )

Now we show $\{x_{n}\}$ cons. indeed:

- Since $x_{n}>0$, we see $x_{n+1}=\frac{x_{n}}{2}+\frac{1}{x_{n}} \geqslant \sqrt{\frac{1}{2}}=\frac{\sqrt{2}}{2}$ for all $n$

- $x_{n+1}-x_{n}=\frac{2-x_{n}^{2}}{2 x_{n}} \leqslant 0$

Thus, $\{x_{n}\}$ is non-increasing and bounded from below by $\frac{\sqrt{2}}{2}$, and therefore it must converge
