# MA127-2023春 期中考试答案

## 一、选择题答案

### (1)

$\vec{n}_{1}=(1,2,-1), \quad \vec{n}_{2}=(1,1,0)$

$\Rightarrow \quad \cos \theta=\frac{\vec{n}_{1} \cdot \vec{n}_{2}}{\left|\vec{n}_{1}\right| \cdot\left|\vec{n}_{2}\right|}=\frac{3}{\sqrt{6} \cdot \sqrt{2}}=\frac{\sqrt{3}}{2}$

$\Rightarrow \theta=\frac{\pi}{6}$ **（答案D）**

### (2)

$V(t)=(\sqrt{t},-\sqrt{2-t}, 1), \quad|V(t)|=\sqrt{3}$

$\Rightarrow L=\int_{\frac{1}{4}}^{\frac{1}{2}}|v(t)| d t=\frac{\sqrt{3}}{4}$ **（答案C）**

### (3)

$\lim\limits_{(x, y) \rightarrow(0,1)} \frac{\ln (1+x y)}{x}=\lim\limits_{(x, y) \rightarrow(0,1)} \frac{\ln (1+x y)}{x y} \cdot y \Rightarrow \lim\limits_{y \rightarrow 1} y=1$

$a=1$ 时，$f(0,1)=a=1$。$\Rightarrow \lim\limits_{(x, y) \rightarrow (0,1)} f(x,y)=f(0,1)$ **（答案C）**

### (4) . $0 \leqslant a_{n} \leqslant \frac{1}{n}$ .(4A

(A) .$\sum_{n=1}^{\infty}(-1)^{n} \frac{a_{n}}{(1+\ln n)^{2}} \therefore 0 \leq\left|(-1)^{n} \frac{a_{n}}{(1+\ln n)^{2}}\right| \leq \frac{1}{n(1+\ln n)^{2}}$

而 $f(x)=\frac{1}{x(1+\ln x)^{2}}>0$,, 连渎 $(x \geqslant 1)$

日 $\int_{1}^{\infty} \frac{1}{x(\ln (t+1+1)^{2}} d x=\int_{1}^{\infty} \frac{d(1+\ln x)}{(1+\ln x)^{2}}$

$=-\frac{1}{1+\ln x}]_{1}^{\infty}$

$\Rightarrow \sum_{n=1}^{\infty} \frac{1}{n(1+\tan n)^{2}} 4<$

$=1.42$

$\Rightarrow \sum(-1)^{n} \frac{a_{n}}{(1+\ln n)^{2}}$ 他对收领, 故收领.

(B) .$\sum_{n=1}^{\infty}(-1)^{n} a_{n}$ : 令 $a_{n}=\frac{(-1)^{n}+1}{7 n}$ 则 $0 \leq a_{n} \leq \frac{1}{n}$

$$
\begin{aligned}
\text { 且 } \begin{aligned}
& \sum_{n=1}^{\infty}(-1)^{n} a_{n}=\sum_{n=1}^{\infty} \frac{1+(-1)^{n}}{2 n} \\
&=\sum_{n=1}^{\infty}(\frac{1}{2 n}+\frac{(-1)^{n}}{2 n}) \\
& \Rightarrow \text { 岁 发 }
\end{aligned}
\end{aligned}
$$

(C) $a_{n}=\frac{1}{2 n} .0<a_{n}<\frac{1}{n}$ .但 $\sum a_{n}$ 发.

(D) .$a_{n}=\frac{(-1)^{n}+1}{2 n}$

$$
\begin{aligned}
\Rightarrow \sum(-1)^{n} \frac{a_{n}}{1+\ln n} & =\sum \frac{(-1)^{n}+1}{2 n(\ln n * 1)} \\
& =\sum(\frac{(-1)^{n}}{2 n(\ln n+1)}+\frac{1}{2 n(\ln n+1)})
\end{aligned}
$$

对于 $\sum_{n=1}^{\infty} \frac{(-1)^{n}}{2 n(\ln n+1)}: \frac{1}{2 n(\ln n+1)} \rightarrow, \rightarrow 0, \Rightarrow$ 收故

对于 $\sum_{n=1}^{\infty} \frac{1}{2 n(\ln n+1)}: \quad \sum_{n \rightarrow \infty} \frac{\frac{1}{2 n(\ln n+1)}}{\frac{1}{n \ln n}}=\frac{1}{2}$

而 $\sum_{n=2}^{\infty} \frac{1}{n \ln n} 4_{2} \Rightarrow \sum_{n=2}^{\infty} \frac{1}{2 n(\ln n+1)} 4_{2}^{\prime}$

$$
\Rightarrow \sum_{n=1}^{\infty} \frac{1}{2 n(\ln n+1)} \text { 发 }
$$

(5) .古 $\sum_{n=1}^{\infty} a_{n} x^{n}$ 在 $x=-2$ 处收(C)

则 $\Rightarrow|x|<2$ 日ま, $\sum_{n=1}^{\infty} a_{n} x^{n}$ 秉对收领

$\Rightarrow|x|<2$ 时, $(\sum_{n=1}^{\infty} a_{n} x^{n})^{\prime}\{$ 促对收做.

$$
\sum_{n=1}^{\infty} n a_{n} x^{n-1}
$$

$\Rightarrow x=1$ 时, $\sum_{n=1}^{\infty} n a_{n} x^{n-1}=\sum_{n=1}^{\infty} n a_{n}$ 收领

(2) . (1). $r=\csc \theta e^{r \cos \theta}$ $\Rightarrow r \sin \theta=e^{r \cos \theta} \Rightarrow y=e^{x}$

(2) . $d=\frac{|1+2+3+4|}{\sqrt{1+2^{2}+3^{2}}}=\frac{10}{\sqrt{14}}$

(3) . $v(t)=\int_{0}^{t} a(x) d x+v(0)=(e^{x}]_{0}^{t}, \frac{x^{2}}{2}]_{0}^{t},-\frac{1}{2} \cos 2 x]_{i}^{t})$

$$
\begin{aligned}
& a(t)=(e^{t}, t, \sin 2 t)=(e^{t}-1, \frac{t^{2}}{2},-\frac{1}{2} \cos 2 t+\frac{1}{2})+(1,0,0)+(1,0,0) \\
& +(1,0,0) \\
& =(e^{+}, \frac{t^{2}}{2}, \frac{1}{2}-\frac{1}{2} \cos 2 t) \\
& \Rightarrow \gamma(t)=\int_{0}^{t} v(x) d x+r(0) \\
& =(e^{t}-1, \frac{t^{3}}{6}, \frac{t}{2}-\frac{1}{4} \sin 2 t) . \\
& \text { (4). } \sin x=x-\frac{x^{3}}{3!}+\cdots \\
& \Rightarrow{\underset{x \rightarrow 0}{ }}_{l_{x \rightarrow 0}} \frac{3 \sin (2 x)-2 \sin (3 x)}{6 x^{3}+x^{4}} \\
& =\lim\limits_{x \rightarrow 0} \frac{3(2 x-\frac{(2 x)^{3}}{3!}+0(x^{3}))-2(3 x-\frac{(3 x)^{3}}{3!}+0(x^{3}))}{6 x^{3}+x^{4}} \\
& =\varliminf_{x \rightarrow 0} \frac{(-4+9) x^{3}+o(x^{3})}{6 x^{3}+x^{4}}=\frac{5}{6} \text {. } \\
& \text { (5). } S=\sum_{n=1}^{\infty} \frac{(-\ln 2)^{n}}{n!}
\end{aligned}
$$

3.$\sum_{n=1}^{\infty} \frac{\ln \eta}{n}(x-1)^{n}$

(1) .$\ell_{n \rightarrow \infty}\left|\frac{\ln (n+1) \cdot(x-1)^{n+1}}{n+1} \cdot \frac{n}{\ln n \cdot(x-1)^{n}}\right|$

$=l_{n \rightarrow \infty}\left|\frac{\ln (n+1)}{\ln n} \cdot \frac{n}{n+1}\right| \cdot|x-1|=|x-1|<1$ 肘, $\sum_{n=1}^{\infty} \frac{\ln n}{n}(x-1)^{n}$ 绝收

$x=$ 日时 $\Rightarrow \sum_{n=1}^{\infty}(-1)^{n} \frac{\ln n}{n}: \quad f(x)=\frac{\ln x}{x}$

Shift

$$
f^{\prime}(x)=\frac{1-\ln x}{x^{2}}<0(x \geqslant 3)
$$

$$
\Rightarrow n \geqslant 3,\left\{\frac{\ln n}{n}\right\} b \text {, 且 } \frac{l_{n \rightarrow \infty}}{} \frac{\ln n}{n}=0 \text {. }
$$

$\Rightarrow \sum_{n=1}^{\infty}(-1)^{n} \frac{\ln n}{n}$ 收

$x=2$ 肘 $\Rightarrow \sum_{n=1}^{\infty} \frac{\ln n}{n}: f(x)=\frac{\ln x}{x}>0, \zeta(x \geqslant 3)$, 连卖

且 $\left.\int_{3}^{\infty} \frac{\ln x}{x} d x=\frac{1}{2}(\ln x)^{2}\right]_{3}^{\infty}=\infty$, 发

$$
\Rightarrow \sum_{n=3}^{\infty} \frac{\ln n}{n} 发散 \Rightarrow \sum_{n=1}^{\infty} \frac{\ln n}{n} 发散
$$

$\Rightarrow$ 收敛域:  $0 \leq x<2$ or $[0,2$ ).

(2). $0<x<2$ 时, 绝对收敛

而对于 $x=0$ 时, $\sum_{n=1}^{\infty}(-1)^{n} \frac{\ln n}{n}: \quad \sum_{n=1}^{\infty}\left|\frac{(-1)^{n} \ln n}{n}\right|=\sum_{n=1}^{\infty} \frac{\ln n}{n}$ 发散.

$\Rightarrow x=0$ 时, 条件收敛.

4.(1) $\lim\limits_{(x, y) \geqslant 10,0)} \frac{y^{2} \sin ^{2} x}{x^{4}+y^{4}}$

Sol.不存在

$$
\begin{aligned}
\text { 令 } y=k x(k \neq 0) . \text { 上戒 } & =\frac{k_{x \rightarrow 0}}{} \frac{k^{2}}{(1+k^{4})} \cdot \frac{x^{2} \cdot \sin ^{2} x}{x^{4}} \\
& =l_{x \rightarrow 0} \frac{k^{2}}{1+k^{4}} \cdot \frac{\sin ^{2} x}{x^{2}}=\frac{k^{2}}{1+k}
\end{aligned}
$$

(2)

$$
\begin{aligned}
&\left|\frac{2 x y}{\sqrt{x^{2}+2 y^{2}}}\right|=\left|\frac{x}{\sqrt{x^{2}+2 y^{2}}} \cdot 2 y\right| \\
& \leq 2|y| \\
&x, y) \rightarrow(0,0) \text { 时, } 2|y| \rightarrow 0 \Rightarrow \frac{l}{(x, y) \rightarrow(0,0)} \frac{2 x y}{\sqrt{x^{2}+2 y^{2}}}=0
\end{aligned}
$$

5.$L_{1}=\left\{\begin{array}{l}x=t \\ y=1 \\ z=1+t .\end{array}\right.$

$l_{z}:\left\{\begin{array}{l}x=1+25 \\ y=0 \\ z=25 .\end{array}\right.$

$\Rightarrow \quad \tau_{1}^{1}=(1,0,1) . \quad \tau_{2}=(2, v, 2)$

$\Rightarrow \tau_{2}^{\prime}=2 \tau_{1}^{\prime} \quad \Rightarrow \quad L_{1} \| L_{2}$

$\Rightarrow$ 存在平面 M 过 $L_{1} S L_{2}$.

在 4 上取点 $A(0,1,1)$, 在 $L_{2}$ 上取一点 $B(1,0,0)$

$\Rightarrow \overrightarrow{A B}=(1,-1,-1)$

$\vec{n}_{n}=\left|\begin{array}{ccc}i & j & k \\ 1 & 0 & 1 \\ 1 & -1 & -1\end{array}\right|=(1,2,-1), M \notin$ 点 $B(1,0,0)$

$\Rightarrow$ 平面 $M$ 为: $(x-1)+2 y-z=0$

邵 $x+2 y-z=1$

6. $0<b<a<1$

(l)

$$
0<\frac{C_{n}}{\sqrt{(1+a^{n})(1+b^{n})}} \leqslant a^{n}
$$

而 $0<a<1, \sum_{n=1}^{\infty} a^{n} 4<\Rightarrow \sum_{n=1}^{\infty} \frac{c_{n}}{\sqrt{(1+a^{n})(1+b^{n})}} 4<$

$$
\begin{aligned}
& \text { (2) } \\
& (\frac{a^{n}}{n^{2}})^{\frac{1}{n}}<(\frac{a^{n}}{n^{2}}+\frac{b^{n}}{n})^{\frac{1}{n}} \leqslant(\frac{2 a^{n}}{n})^{\frac{1}{n}} \text {. } \\
& \begin{aligned}
\lim\limits_{n \rightarrow \infty}(\frac{a^{n}}{n^{2}})^{\frac{1}{n}} & =h_{n \rightarrow \infty} \frac{a}{(n^{\frac{1}{n}})^{2}}, h_{n \rightarrow \infty}(\frac{2 a^{n}}{n})^{\frac{1}{n}}=l_{n \rightarrow \infty} \frac{2^{\frac{1}{n}} \cdot a}{n^{\frac{1}{n}}}=a . \\
& =a
\end{aligned} \\
& \Rightarrow l_{n \rightarrow \infty}(\frac{a^{n}}{n^{2}}+\frac{b^{n}}{n})^{\frac{1}{n}}=a \text {. }
\end{aligned}
$$

7.$r(t)=(\sqrt{2} \cos t, \sin t, \sin t)$

(A)

Sol.$\quad V(t)=(-\sqrt{2} \sin t, \cos t, \cos t)$

$$
\begin{aligned}
& |v(t)|=\sqrt{2 \sin ^{2} t+\cos ^{2} t+\cos ^{2} t}=\sqrt{2} \\
\Rightarrow & T(t)=\frac{v}{|v|}=\frac{1}{\sqrt{2}}(-\sqrt{2} \sin t, \cos t, \cos t) \\
\Rightarrow & \frac{d 7}{d t}(t)=\frac{1}{\sqrt{2}}(-\sqrt{2} \cos t,-\sin t,-\sin t)
\end{aligned}
$$

而 $\left|\frac{d T}{d t}\right|=\frac{1}{\sqrt{2}} \sqrt{2 \cos ^{2} t+\sin ^{2} t+\sin ^{2} t}=1$

$\Rightarrow N(t)=\frac{d 7}{d t}=\frac{1}{\sqrt{2}}(-\sqrt{2} \cos t,-\sin t,-\sin t)$

(B) .$\quad k(t)=\frac{1}{|v(t)|} \cdot\left|\frac{d T}{d t}\right|=\frac{1}{\sqrt{2}}$

8.$f(x)=\frac{4}{x^{2}-2 x+5}+\ln x$

$$
\begin{aligned}
& =\frac{4}{(x-1)^{2}+4}+\ln (1+(x-1)) \\
& =\frac{1}{1+\frac{(x-1)^{2}}{4}}+\ln [1+(x-1)] \\
& \text { 而 } \frac{1}{1+\frac{(x-1)^{2}}{4}}=\sum_{n=0}^{\infty}\left[-\frac{(x-1)^{2}}{4}\right]^{n}=\sum_{n=0}^{\infty} \frac{(-1)^{n}}{4^{n}} \cdot(x-1)^{2 n},\left|\frac{(x-1)^{2}}{4}\right|<1 . \\
& \ln [1+(x-1)]=\sum_{n=1}^{\infty} \frac{(-1)^{n-1}(x-1)^{n}}{n},-1 \leqslant x-1<1 \text { 即 } 0 \leqslant x<2
\end{aligned}
$$

$\Rightarrow x \in(0,2)$ 日寸, $f(x)=\sum_{n=0}^{\infty} \frac{(-1)^{n}}{4^{n}}(x-1)^{2 n}+\sum_{n=1}^{\infty} \frac{(-1)^{n-1}(x-1)^{n}}{n}$,

