一(1)A

$$
\begin{array}{ll}
f(x-a z, y-b z)=0 & \Rightarrow
\end{array} \begin{array}{ll}
u=x-a z \\
v=y-b z & \\
y, z)=f(a x-a z, y-b z)=0 & f_{u}\left(1-a \frac{\partial z}{\partial x}\right)+f_{v}\left(-\frac{\partial z}{\partial x}\right)+f_{v}\left(1-b \frac{\partial z}{\partial y}\right)=0 \Rightarrow\left(a f_{u}+b f_{v}\right) \frac{\partial z}{\partial x}=f_{u} \\
&
\end{array}
$$

or $F(x, y, z)=f(a x-a z, y-b z)=0$

$\Rightarrow: \frac{\partial z}{\partial x}=-\frac{F_{x}}{F_{z}}, \frac{\partial z}{\partial y}=-\frac{F_{y}}{F_{z}} \Rightarrow a \frac{\partial z}{\partial x}+b \frac{\partial z}{\partial y}=a \cdot \frac{f_{u}}{a f_{u}+b f_{v}}+b \cdot \frac{f_{v}}{a f_{u}+b f_{v}}=1$

$F_{z}=-a f_{u}-t f_{v}, F_{x}=f_{u}, F_{y}=f_{v} \Rightarrow$

(2) $C$

(2) $n>0, a_{n}>0 . \quad \lim\limits_{n \rightarrow \infty} n a_{n}=\lim\limits_{n \rightarrow \infty} \frac{a_{n}}{\frac{1}{n}}=1 \neq 0 \ldots, \sum \frac{1}{n}$ diverges $\Rightarrow \sum a_{n}$ diverges

(3) $B$

$2 x^{2}+y^{2}=z^{2}$ 椭圆锥.

$$
\begin{array}{rlrl}
f(x, y) & =\varphi(x+y)+\varphi(x-y)+\int_{x-y}^{x+y} \psi(t) d t . & \text { let } \begin{array}{l}
x+y=u \\
x-y=v
\end{array} \\
\Rightarrow \frac{\partial f}{\partial x} & =\varphi_{u}+\varphi_{v}+\psi(x+y)-\psi(x-y) \quad & \frac{\partial f}{\partial y^{\prime}}=\varphi_{u} \varphi_{v}+\psi(x+y)+\psi(x-y) \\
\frac{\partial f}{\partial x^{2}} & =\varphi_{u u}+\varphi_{v u}+\psi_{u}(x+y)-\psi_{v}(x-y) \quad \frac{\partial^{2} f}{\partial y^{2}}=\varphi_{u u}+\varphi_{u}+\psi_{u}(x+y)-\psi_{v}(x-y) \\
& \Rightarrow \frac{\partial f}{\partial x^{2}}=\frac{\partial^{2} f}{\partial y^{2}} &
\end{array}
$$

$\lim\limits_{x, y) \rightarrow(0,0)}(1+x y)^{\frac{1}{x^{2}+y^{2}}}=\lim\limits_{x \rightarrow 0}\left(1+x^{2}\right)^{\frac{1}{x^{2}}}=\lim\limits_{x \rightarrow 0}\left[\left(1+x^{2}\right)^{\frac{1}{x^{2}}}\right]^{\frac{1}{2}}=e^{\frac{1}{2}} \Rightarrow$

$\Rightarrow$ dees not exist

$\lim\limits_{\substack{(x, y) \rightarrow(0,0) \\ y=-x}}(1+x y)^{\frac{1}{x^{2}+y^{2}}}=\lim\limits_{x \rightarrow 0}\left(1-x^{2}\right)^{\frac{1}{2 x^{2}}}=\lim\limits_{x \rightarrow 0}\left[\left(1-x^{2}\right)^{\frac{1}{-x^{2}}}\right]^{\frac{1}{-2}}=e^{\frac{1}{-2}}$

(I)

$$
\begin{aligned}
& =\text { (1) } \frac{-\frac{3}{2}}{\vec{a}+\vec{b}+\vec{c}=\overrightarrow{0}} \\
& \Rightarrow \left\lvert\, \begin{array}{l}
|\vec{a}|^{2}+\vec{a} \cdot \vec{b}+\vec{a} \cdot \vec{c}=0 \\
\vec{a} \cdot \vec{b}+|\vec{b}|^{2}+\vec{b} \cdot \vec{c}=0 \\
\vec{a} \cdot \vec{c}+\vec{b} \cdot \vec{c}+|\vec{c}|^{2}=0
\end{array}\right
\end{aligned}
$$

(1)

(2)

(1) + (2)+ (3)$\Rightarrow 2(\vec{a} \cdot \vec{b}+\vec{a} \cdot \vec{c}+\vec{b} \cdot \vec{c})=-3$

$$
\Rightarrow \vec{a} \cdot \vec{b}+\vec{b} \cdot \vec{c}+\vec{c} \cdot \vec{a}=-\frac{3}{2}
$$

(2) $2 \vec{i}-4 \vec{i}+6 \vec{k}$

(1)

$\therefore \vec{c}+\vec{c}+\vec{c}+\vec{a} \times \vec{a}\left|=\vec{a}+\vec{i}+\begin{array}{ccc}\vec{i} & \vec{j} & \vec{k} \\ 1 & 2 & 1 \\ -1 & 1 & 1\end{array}\right|=\vec{i}-2 \vec{j}+3 \vec{k}$

2)$\quad \Rightarrow \vec{c}=K(1,-2 \times 3)$ of $x$

$$
\because \vec{c} \cdot(\vec{\imath}-2 \vec{j}+\vec{k})=16 \Rightarrow 8 k=16 \Rightarrow k=2 \Rightarrow \vec{c}=(2,-4,6)
$$

(3) . 1

Since $\sum_{n=2}^{\infty}\left(\tan \frac{1}{n}-k \ln \left(1-\frac{1}{n}\right)\right)$ converges, let $x=\frac{1}{n}, n \rightarrow \infty \Rightarrow x \rightarrow 0$

$\Rightarrow \quad \lim\limits_{x \rightarrow 0}\left|\frac{\tan x-k \ln (1-x)}{x^{p}}\right|=c \geqslant 0, p>1$

$$
\Rightarrow \lim\limits_{x \rightarrow 0}\left|\frac{\sec ^{2} x}{p x^{p-1} \rightarrow 0}+\frac{k}{1-x}\right|=c \geqslant 0, p>\mid \omega_{1} p x^{p-1} \rightarrow 0
$$

$$
\Rightarrow 1+k \rightarrow 0 \Rightarrow k=-1
$$

8 (when $k=-1 \quad \lim\limits_{x \rightarrow 0} \frac{\tan x+\ln (1-x)}{x^{p}}=\lim\limits_{x \rightarrow 0} \frac{\sec ^{2} x-\frac{1}{1-x}}{p x^{p-1}}=\lim\limits_{x \rightarrow 0} \frac{(1-x)^{s^{2}} x-1}{p x^{p-1}}=$

$$
=\lim\limits_{x \rightarrow 0} \frac{-\sec ^{2} x+2(1-x) \sec ^{2} x \tan x}{p(p-1) x^{p-2}}=\lim\limits_{x \rightarrow 0} \frac{-1+2(1-x) \tan x \rightarrow-1 \neq 0}{p(p-1) x^{p-2}} \Rightarrow p-2=0
$$

14)

$$
\begin{aligned}
& f=y(x)=\sin x \Rightarrow f^{\prime}(x)=\cos x, f^{\prime \prime}(x)=-\sin x \\
& k=\frac{\left|f^{\prime \prime}(x)\right|}{\left(1+\left(f^{\prime}(x)\right)^{2}\right)^{\frac{3}{2}}}=\frac{|-\sin x|}{\left(1+\cos ^{2} x\right)^{\frac{3}{2}}}=\frac{|\sin x|}{\left(2-\sin ^{2} x\right)^{\frac{3}{2}}}
\end{aligned}
$$

when $\mid \sin x$ max, $\sin ^{2} x$ is max

$$
\begin{array}{ll}
\Rightarrow 2-\sin ^{2} x \text { is min. } & \Rightarrow|\sin x| \cdot \frac{1}{\left(2-\sin ^{2} x\right)^{\frac{3}{2}}} \text { is max } \\
\Rightarrow\left(2-\sin ^{2} x\right)^{\frac{3}{2}} \text { is min. } \\
\Rightarrow \frac{1}{\left(2-\sin ^{2} x\right)^{\frac{3}{2}}} \text { is max } & \Rightarrow k \text { is max } \\
& \Rightarrow|\sin x|=1 \Rightarrow k=1
\end{array}
$$

(5) $2-2 \ln 2$

$$
\begin{aligned}
\left(z^{2}+y\right)^{x}=x y & \Rightarrow x \ln (z+y)=\ln x y \\
& \Rightarrow \ln (z+y)+x \cdot \frac{1}{z+y} \cdot \frac{\partial z}{\partial x}=\frac{1}{x y} \cdot y \\
& \text { let } x=1, y=2 \cdot z=0 \\
& \Rightarrow \ln 2+\frac{1}{2} \cdot \frac{\partial z}{\partial x}=1 \Rightarrow \frac{\partial z}{\partial x}=2-z \ln 2
\end{aligned}
$$

or let $F(x, y, z)=x \ln (z+y)-\ln x y$

$$
\begin{aligned}
\Rightarrow \quad F_{x} & =\ln (z+y) \\
F_{z} & =\frac{x}{z+y}=\frac{x}{2}=\ln 2-1 \\
\Rightarrow \frac{\partial z}{\partial x} & =-\frac{F_{x}}{F z}=2-2 \ln 2
\end{aligned}
$$

$$
\begin{aligned}
A & =\int_{-\frac{\pi}{2}}^{\frac{\pi}{2}} \frac{1}{2}\left[a^{2}(1+\cos \theta)^{2}-a^{2}\right] d \theta \text { or } A=2 \int_{0}^{\frac{\pi}{2}} \frac{1}{2}\left[a^{2}(1+\cos \theta)^{2}-a^{2}\right] d \theta \\
& =\int_{-\frac{\pi}{2}}^{\frac{\pi}{2}} \frac{1}{2}\left[2 a^{2} \cos \theta+a^{2} \cos ^{2} \theta\right] d \theta \\
& =\int_{-\frac{\pi}{2}}^{\frac{\pi}{2}} \frac{1}{2}\left[2 a^{2} \cos \theta+a^{2} \cdot \frac{1+\cos 2 \theta}{2}\right] d \theta . \\
& \left.=\frac{1}{2}\left(2 a^{2} \sin \theta+\frac{1}{2} a^{2} \theta+\frac{a^{2}}{4} \sin 2 \theta\right)\right]_{-\frac{\pi}{2}}^{\frac{\pi}{2}} \\
& =2 a^{2}
\end{aligned}
$$

$$
\begin{aligned}
\left.A_{1}\right) & =2 \int_{0}^{\pi} \frac{1}{2}\left[a^{2}(1+\cos \theta)^{2}\right] \\
& =\int_{0}^{\pi}\left(a^{2}+2 a^{2} \cos \theta+a^{2} \cos ^{2} \theta\right) d \theta . \\
& =\int_{0}^{\pi}\left(a^{2}+2 a^{2} \cos \theta+a^{2} \cdot \frac{(+\cos \theta}{2}\right) d \theta . \\
& \left.=a^{2} \theta+2 a^{2} \sin \theta+\frac{a^{2}}{2} \theta+\frac{a^{2}}{4} \sin 2 \theta\right]_{0}^{\pi} \\
& =\frac{3}{2} a^{2} \pi \\
\Rightarrow & A_{2}=A_{1}-A=\frac{3}{2} a^{2} \pi-\left(2+\frac{\pi}{4}\right) a^{2}=\frac{5}{4} \pi a^{2}-2 a^{2}=\left(\frac{5}{4} \pi-2\right) a^{2}
\end{aligned}
$$

4. $\vec{r}(t)=f(t) \vec{i}+g(t) \vec{j}+h(t) \vec{k}$., $f(t)=\int_{0}^{t} \cos \left(x^{2}\right) d x, g(t)=-t \cos t$

$$
\begin{aligned}
h(t) & =\sum_{n=1}^{\infty} t^{n} \\
\Rightarrow h^{\prime}(t) & =\sum_{i=1}^{\infty} t^{n-1}=\sum_{n=0}^{\infty} t^{n}=\frac{1}{1-t} \\
f^{\prime}(t) & =\cos \left(t^{2}\right) \\
g^{\prime}(t) & =-\cos t+t \sin t
\end{aligned}
$$

$\Rightarrow f^{\prime}(0)=1, \quad g^{\prime}(0)=-1, \quad h^{\prime}(0)=1$

$\Rightarrow f^{\prime}(0)=(1,-1,1)$

5. (1) $f(x, y)=\left\{\begin{array}{cc}y \sin \frac{1}{x^{2}+y^{2}} & ,(x, y) \neq(0,0) \\ 0 & ,(x, y)=(0,0)\end{array}\right.$

$$
\begin{array}{r}
\lim\limits_{(x, y) \rightarrow(0,0)} f(x, y)=\lim\limits_{(x, y) \rightarrow(0,0)} y \sin \frac{1}{x^{2}+y^{2}}=0 \text { since }\left|\sin \frac{1}{x^{2}+y^{2}}\right| \leqslant 1 \\
0 \leqslant|f(x, y)| \leqslant|y| \rightarrow 0
\end{array}
$$

(2) $f_{x}(0,0)=\lim\limits_{h \rightarrow 0} \frac{f(h, 0)-f(0,0)}{h}=\lim\limits_{h \rightarrow 0} \frac{0-0}{h}=0$

$$
f_{y}(0,0)=\lim\limits_{h \rightarrow 0} \frac{f(0, h)-f(0,0)}{h}=\lim\limits_{h \rightarrow 0} \frac{h \sin h h^{-0}}{h}=\lim\limits_{h \rightarrow 0} \sin \frac{1}{h^{2}} \text { does nt exist. }
$$

6.(1) $\lim\limits_{(x, y) \rightarrow(0,0)} \frac{x y}{\sqrt{x^{2}+y^{2}}}=\lim\limits_{r \rightarrow 0} \frac{r^{2} \cos \theta \sin \theta}{|r|}=\lim\limits_{r \rightarrow 0}|r| \cos \theta \sin \theta=0$. since |cos $\theta \sin \theta \mid \leqslant 1$. or $0 \leqslant\left|\frac{x^{y}}{\sqrt{x^{2}+y^{2}}}\right| \leqslant|y| \rightarrow 0$

(2) $\lim\limits_{(x, y) \rightarrow(0,0)} \frac{x y^{3}+2 x^{2} y^{4}}{x^{2}+y^{6}}=\lim\limits_{(x, y) \rightarrow(0,0)} \frac{k y^{6}+2 k^{2} y^{7}}{k^{2} y^{6}+y^{6}}=\lim\limits_{\substack{ \\y \rightarrow 0}} \frac{k+2 k^{2} y}{k^{2}+1}=\frac{k}{k^{2}+1}$ $x=k y^{\prime} ;$ $\Rightarrow$ the limit does not exist

T. (1) $f(x)=\sum_{n=1}^{\infty} \frac{n+2}{n(n+1)} x^{n}$

$$
\left|\frac{u_{n+1}}{u_{n}}\right|=\left|\frac{(n+3)}{(n+2)(n+1),(n+2)} x\right| \rightarrow|x|<1 \Rightarrow-1<x<1
$$

when $x=1 \quad \sum_{n=1}^{\infty} \frac{n+2}{n(n+1)}$ diverges since $\frac{\frac{n+2}{n(n+1)}}{\frac{1}{n}} \rightarrow 1, \sum \frac{1}{n}$ diverges

when $x=-1, \quad \sum_{n=1}^{\infty}(-1)^{n} \frac{n+2}{n(n+1)}$ converges conditionally. Sine $\sum \frac{n+2}{n(n+1)}$ diverges

$$
\Rightarrow[-1,1]
$$

$$
a_{n}=\frac{n+2}{n(n+1)}>0 \rightarrow 0
$$

(2) $f(x)=\sum_{n=1}^{\infty} \frac{n+2}{n(n+1)} x^{n}=\sum_{n=1}^{\infty} \frac{x^{n}}{n+1}+\sum_{n=1}^{\infty} \frac{2}{n(n+1)} x^{n}=\sum_{n=1}^{\infty} \frac{x^{n}}{n+1}+2 \sum_{n=1}^{\infty} \frac{x^{n}}{n}-2 \sum_{n=1}^{\infty} \frac{x^{n}}{n+1}=2 \sum_{i=1}^{\infty} x^{n} \frac{\sum_{n}^{n}}{n} \frac{x^{n} x^{n}}{}$

$$
g(x)=\sum_{n=1}^{\infty} \frac{x^{n}}{n+1}=\frac{1}{x} \sum_{n=1}^{\infty} \frac{x^{n+1}}{n+1},\left(\sum_{n=1}^{\infty} \frac{x^{n+1}}{n+1}\right)^{\prime}=\sum_{n=1}^{\infty} x^{n}=\frac{x}{1-x}
$$

if $x \neq 0$

$$
\begin{aligned}
\Rightarrow \sum_{n=1}^{\infty} \frac{x^{n+1}}{n+1} & =\int \frac{x}{1-x} d x=\int \frac{1-(1-x)}{1-x} d x=\int \frac{d x}{1-x}-x \\
& =-\ln (1-x)-x+c \\
\text { let } x=0 . & \Rightarrow c=0
\end{aligned}
$$

$\Rightarrow g(x)=-\frac{\ln (1-x)}{x}-1$, if $x \neq 0$

$$
\begin{aligned}
& \quad h(x)=\sum_{n=1}^{\infty} \frac{x^{n}}{n}{ }^{n} \Rightarrow h^{\prime}(x)=\sum_{n=1}^{\infty} x^{n-1}=\frac{1}{1-x} \Rightarrow h(x)=-\ln (1-x) \\
& \Rightarrow \\
& f(x)= \begin{cases}-2 \ln (1-x)+\frac{\ln (1-x)}{x}+1=1+\left(\frac{1}{x}-2\right) \ln (1-x), & x \neq 0 . \\
0 . & x=0 .\end{cases}
\end{aligned}
$$

8. $\sum_{n=2}^{\infty} \frac{(-1)^{p+1}}{n^{p}(\ln n)^{2}}, p>0$. Let $u_{n}=\frac{1}{n^{p}(\ln \eta)^{2}}\left\{\begin{array}{l}\text { converges absolutely if } p \geqslant 1 \\ \text { converges conditionally if } 0<p<1\end{array}\right.$

![](https://cdn.mathpix.com/cropped/2025_04_21_5ecf81e20af84819e6ffg-6.jpg?height=130&width=1357&top_left_y=1854&top_left_x=364)

(2) if $\left.p=1 \cdot \sum_{n-2}^{\infty} \frac{1}{n(\ln n)^{2}}, f(x)=\frac{1}{x(\ln x)^{2}}, \int_{2}^{\infty} \frac{d x}{x(\ln x)^{2}}=-\frac{1}{\mid n x}\right]_{2}^{\infty}=\frac{1}{\ln 2}$ converges $\Rightarrow \sum u_{n}$ ca query

![](https://cdn.mathpix.com/cropped/2025_04_21_5ecf81e20af84819e6ffg-6.jpg?height=118&width=1355&top_left_y=2051&top_left_x=330) $\rightarrow \Sigma \mathrm{K}_{n}$ converge concrify

9. $\lim\limits_{n \rightarrow \infty}\left(\left(n^{2}-n\right) e^{\frac{1}{n}}-\sqrt{n^{4}+1}\right)$

lef $f(x)=\left(x^{2}-x\right) e^{\frac{1}{x}}-\sqrt{x^{4}+1}$

$$
\begin{aligned}
& =\left(x^{2}-x\right)\left(1+\frac{1}{x}+\frac{1}{2!x^{2}}+\cdots+\frac{1}{k!x^{k}}+\cdots\right) \\
& =x^{2}-\frac{1}{2}-\frac{1}{3 x}+\cdots
\end{aligned}
$$

$$
\begin{aligned}
\sqrt{x^{4}+1}=x^{2} \sqrt{1+\frac{1}{x^{4}}} & =x^{2}\left(1+\frac{1}{2 x^{4}}-\frac{1}{8 x^{8}}+\cdots\right) \\
& =x^{2}+\frac{1}{2 x^{2}}-\frac{1}{8 x^{6}}+\cdots
\end{aligned}
$$

$$
\begin{aligned}
& \Rightarrow f(x)=-\frac{1}{2}-\frac{1}{3 x}+\cdots \\
& \Rightarrow \lim\limits_{x \rightarrow \infty} f(x)=-\frac{1}{2}
\end{aligned}
$$

