# MA127-2019春 期中考试答案

## 一、判断题

### 1-1

**False**

$\Rightarrow \sum \limits_{n=1}^{\infty} a_{n}$ converges, $a_{n}<0$ for $n>1000$

$\Rightarrow \sum \limits_{n=1}^{\infty}\left|a_{n}\right|=\sum \limits_{n=1}^{1000}\left|a_{n}\right|-\sum \limits_{n=1001}^{\infty} a_{n}$ converges and $\lim\limits_{n \rightarrow \infty} a_{n}=0$

$\therefore \lim\limits_{n \rightarrow \infty}\left|a_{n}\right|=\lim\limits_{n \rightarrow \infty} \frac{a_{n}^{2}}{\left|a_{n}\right|}=0, \sum\left|a_{n}\right|$ converges, $\Rightarrow \sum a_{n}^{2}$ converges.

### 1-2

**True**

$\Rightarrow \sum a_{n}(x-1)^{n}$ converges at $x=0$

$\Rightarrow \sum a_{n}(x-1)^{n}$ converges absolutly for $|x-1| < 1$

so $x-1=-1$, i.e., $0<x<2$

diverges at $x=2$, i.e., $x-1=1$

$\Rightarrow$ diverges for $|x-1|>1$

$\Rightarrow x>2$ or $x<0$ diverges. So converges for $0 \leq x<2$

since. $\sum a_{n} x^{n}$ converges at $x=c \neq 0$

$\Rightarrow$ converges absolutely for all $|x|<|c|$

diverges at $x=d \Rightarrow$ diverges for $|x|>|d|$

or

$\sum a_{n}(x-1)^{n}$ converges at $x=0$

$\Rightarrow \lim\limits_{n \rightarrow \infty} a_{n}=0 \Rightarrow \exists \varepsilon=1$ s.t. $\left|a_{n}\right|<1 \quad \forall n>N$

$\Rightarrow\left|a_{n}(x-1)^{n}\right|<|x-1|^{n}$ for $\forall|x-1|<1$

and $\sum|x-1|^{n}$ converges

$\Rightarrow \sum|a_{n}(x-1)^{n}|$ converges for $|x-1|<1 \Rightarrow 0<x<2$

$\Rightarrow$ converges at $0 \leq x<2$

### 1-3

**True**

Since

$f_{x}(x_{0}, y_{0})=\lim\limits_{x \rightarrow x_{0}} \frac{f(x, y_{0})-f(x_{0}, y_{0})}{x-x_{0}}=c$ exists

and $x-x_{0} \rightarrow 0 \Rightarrow \lim\limits_{x \rightarrow x_{0}} f(x, y_{0})=f(x_{0}, y_{0})$

$f_{y}(x_{0}, y_{0})=\lim\limits_{y \rightarrow y_{0}} \frac{f(x_{0}, y)-f(x_{0}, y_{0})}{y-y_{0}}$ exist

and $\lim\limits_{y \rightarrow y_{0}}(y-y_{0})=0 \Rightarrow \lim\limits_{y \rightarrow y_{0}} f(x_{0}, y)=f(x_{0}, y_{0})$

$\therefore \lim\limits_{x \rightarrow x_{0}} f(x, y_{0})=\lim\limits_{y \rightarrow y_{0}} f(x_{0}, y)=f(x_{0}, y_{0})$

### 1-4

**True**

$\vec{r}(t) \cdot \frac{d \vec{r}}{d t}=0 \Rightarrow (\vec{r}(t) \cdot \vec{r}(t))^{\prime}=2 \vec{r}(t) \cdot \frac{d \vec{r}}{d t}=0$

$$\Rightarrow |\vec{r}(t)|=c \Rightarrow |\vec{r}(t)|=\text{constant}$$

### 1-5

**False**

For unit circle: $x^{2}+y^{2}=1 \Rightarrow$

$$
\left
\{\begin{array}{l}
x=\cos t \\
y=\sin t
\end{array}
\right.
\Rightarrow
\vec{r}(t)=(\cos t) \vec{i}+(\sin t) \vec{j}
$$

$\vec{T}=\vec{v}=(-\sin t) \vec{i}+(\cos t) \vec{j}$

$\left|\frac{d \vec{T}}{d t}\right|=1,|\vec{v}(t)|=1 \Rightarrow \kappa=1$

For $y=x^{2} \Rightarrow y^{\prime}=2 x, \quad y^{\prime\prime}=2 \Rightarrow y^{\prime}(0)=0, y^{\prime\prime}(0)=2$

$$\kappa=\frac{|y^{\prime\prime}|}{(1+(y^{\prime})^{2})^{3/2}}=\frac{2}{1}=2$$

## 二、多选题

### 2-1

C.

$|\vec{a}+\vec{b}|=\sqrt{|\vec{a}|^{2}+2 \vec{a} \cdot \vec{b}+|\vec{b}|^{2}}=\sqrt{|\vec{a}|^{2}+|\vec{b}|^{2}}$

$|\vec{a}-\vec{b}|=\sqrt{|\vec{a}|^{2}-2 \vec{a} \cdot \vec{b}+|\vec{b}|^{2}}=\sqrt{|\vec{a}|^{2}+|\vec{b}|^2}$

$\therefore |\vec{a}+\vec{b}|=|\vec{a}-\vec{b}|$

### 2-2

D.

$\Rightarrow \vec{v}_{1}=(1,2,-1), \quad \vec{v}_{2}=(-2,1,1) \quad \therefore \vec{v}_{1} \cdot \vec{v}_{2}=-2+2-1=-1, \quad\left|\vec{v}_{1}\right|=\left|\vec{v}_{2}\right|=\sqrt{6}$

$\Rightarrow \cos \theta=-\frac{1}{6}$

But if they intersect:

$$
\left\{
\begin{array}{l}
x = t=1-2t\\
y = 2t=t
\end{array}
\right.
\Rightarrow
\left\{
\begin{array}{l}
t= \frac{1}{3} \\
t = 0
\end{array}
\right.
$$

### 2-3

D

$0 \leq a_{n} < \frac{1}{n} \Rightarrow a_{n}^{2} \leq \frac{1}{n^{2}} \Rightarrow \sum a_{n}^{2}$ converges

$\Rightarrow \sum(-1)^{n} a_{n}^{2}$ converges

## 三

### 3-1

$\Rightarrow \lim \limits_{n \rightarrow \infty} \sqrt[n]{|a_n|}=\lim\limits_{n \rightarrow \infty} \sqrt[n]{(-1)^{n}(1-\frac{1}{n})^{n^{2}}}=\lim\limits_{n \rightarrow \infty}(1-\frac{1}{n})^{n}=e^{-1}<1$

$\Rightarrow$ converges absolutely

### 3-2

$\Rightarrow \lim\limits_{n \rightarrow \infty} e^{-\frac{1}{n}}=e^{0}=1 \neq 0 \Rightarrow$ diverges

### 3-3

$\Rightarrow$ For $\sum \limits_{n=2019}^{\infty} \frac{1}{\sqrt{n^{2}-2019 n+1}}, \lim\limits_{n \rightarrow \infty} \frac{\frac{1}{\sqrt{n^{2}-2019 n+1}}}{\frac{1}{n}}=1, \sum \frac{1}{n}$ diverges $\Rightarrow$ diverges

$u_{n}=\frac{1}{\sqrt{n^{2}-2019 n+1}}>0, \quad u_{n}>u_{n+1}, \quad u_{n} \rightarrow 0 \Rightarrow$ converges conditionally

## 四

### 4-1

$\Rightarrow \left|\frac{u_{n+1}}{u_{n}}\right|=\frac{2^{n+1} \sqrt{n^{2}+n+1}}{2^{n} \sqrt{(n+1)^{2}+(n+1)+1}}|x| \rightarrow 2|x|<1 \Rightarrow|x|<\frac{1}{2} \Rightarrow R=\frac{1}{2}$

### 4-2

when $x=\frac{1}{2}$: $\sum \limits_{n=0}^{\infty} \frac{(-1)^{n+1}}{\sqrt{n^{2}+n+1}}$ converges conditionally since

$\frac{1}{\sqrt{n^{2}+n+1}} > 0, \lim\limits_{n \rightarrow \infty}{\frac{1}{\sqrt{n^{2}+n+1}}} = 0 \\$

$\lim\limits_{n \rightarrow \infty} \frac{1}{\sqrt{n^{2}+n+1}} \cdot n=1, \sum \frac{1}{n}$ diverges

$\Rightarrow \sum \frac{1}{\sqrt{n^{2}+n+1}}$ diverges

when $x=-\frac{1}{2}$

$\sum \limits_{n=0}^{\infty} \frac{(-1)^{n+1} \cdot(-1)^{n}}{\sqrt{n^{2}+n+1}}=\sum \limits_{n=0}^{\infty} \frac{(-1)^{2n+1}}{\sqrt{n^{2}+n+1}}=\sum \limits_{n=0}^{\infty} \frac{-1}{\sqrt{n^{2}+n+1}}$ diverges

$\Rightarrow$ converges absolutely: $\left(-\frac{1}{2}, \frac{1}{2}\right)$, converges: $\left(-\frac{1}{2}, \frac{1}{2}\right]$, converges conditionally: $x=\frac{1}{2}$

## 五

### 5-1

$\frac{d x}{d t}=-3 \cos ^{2} t \sin t, \frac{d y}{d t}=3 \sin ^{2} t \cos t \Rightarrow(\frac{d x}{d t})^{2}+(\frac{d y}{d t})^{2}=9 \sin ^{2} t \cos ^{2} t$

$$
\begin{aligned}
L & =\int_{0}^{\frac{\pi}{2}} \sqrt{(\frac{d x}{d t})^{2}+(\frac{d y}{d t})^{2}} d t=\int_{0}^{\frac{\pi}{2}} \sqrt{9 \sin ^{2} t \cos ^{2} t} d t=\int_{0}^{\frac{\pi}{2}} 3 \sin t \cos t d t \\
&= \frac{3}{2}\sin^{2}t|_{0}^{\frac{\pi}{2}} = \frac{3}{2}
\end{aligned}
$$

### 5-2

$S=\int_{0}^{\frac{\pi}{2}} 2 \pi y \sqrt{(\frac{dx}{d t})^{2}+(\frac{d y}{d t})^{2}} d t=\int_{0}^{\frac{\pi}{2}} 2 \pi \sin ^{3} t \cdot 3 \sin t \cos t d t=\int_{0}^{\frac{\pi}{2}} 6 \pi \sin ^{4} t d \sin t$

=$\frac{6}{5} sin^{5} t |^{\frac{\pi}{2}}_{0} = \frac{6 \pi}{5}$

## 六

$\Rightarrow$ let $P(2,-1,-1), Q(1,0,-1) \Rightarrow \overrightarrow{PQ}=(-1,1,0), \vec{n_{1}}=(2,3,-5)$

$$
\begin{aligned}
\Rightarrow \vec{n}=\overrightarrow{PQ} \times \vec{n_1}=
\left|
\begin{array}{ccc}
\vec{i} & \vec{j} & \vec{k} \\
-1 & 1 & 0 \\
2 & 3 & -5
\end{array}
\right|=-5 \vec{i}-5 \vec{j}-5 \vec{k}
\end{aligned}
$$

$\Rightarrow$ the plane: $-5(x-2)-5(y+1)-5(z+1)=0$

$\Rightarrow x+y+z=0$

## 七

$\Rightarrow$ let $P(1,0,-2), Q(2,-1,3) \Rightarrow \overrightarrow{PQ}=(1,-1,5), \vec{r_{0}}=\vec{i}-2 \vec{k}$

the direction of $\vec{v}(0)$ is $\frac{\overrightarrow{PQ}}{|\overrightarrow{PQ}|}=\frac{1}{\sqrt{27}}(1,-1,5)=\frac{1}{3\sqrt{3}}(1,-1,5)$

So $\vec{v}(0)=|\vec{v}(0)| \cdot \frac{\overrightarrow{PQ}}{|\overrightarrow{PQ}|}=3 \cdot \frac{1}{3\sqrt{3}}(1,-1,5)=\frac{\sqrt{3}}{3}(1,-1,5)$

$$
\begin{aligned}
\vec{a}(t) & =\vec{i}+2 \vec{j}+\vec{k} \\
\Rightarrow \vec{v}(t) & =\int(\vec{i}+2 \vec{j}+\vec{k}) d t=t \vec{i}+2 t \vec{j}+t \vec{k}+\vec{c} \\
\vec{v}(0) & =\frac{\sqrt{3}}{3} \vec{i}-\frac{\sqrt{3}}{3} \vec{j}+\frac{5\sqrt{3}}{3} \vec{k} \\
\Rightarrow \vec{c} & =\frac{\sqrt{3}}{3} \vec{i}-\frac{\sqrt{3}}{3} \vec{j}+\frac{5\sqrt{3}}{3} \vec{k} \\
\Rightarrow \vec{v}(t) & =(t+\frac{\sqrt{3}}{3}) \vec{i}+(2 t-\frac{\sqrt{3}}{3}) \vec{j}+(t+\frac{5\sqrt{3}}{3}) \vec{k} \\
\vec{r}(t) & =\int[(t+\frac{\sqrt{3}}{3}) \vec{i}+(2 t-\frac{\sqrt{3}}{3}) \vec{j}+(t+\frac{5\sqrt{3}}{3}) \vec{k}] d t \\
& =(\frac{1}{2} t^{2}+\frac{\sqrt{3}}{3} t) \vec{i}+(t^{2}-\frac{\sqrt{3}}{3} t) \vec{j}+(\frac{1}{2} t^{2}+\frac{5\sqrt{3}}{3} t) \vec{k}+\vec{c} \\
\vec{r}(0) & =\vec{i}-2 \vec{k} \Rightarrow \vec{c}=\vec{r}(0)=\vec{i}-2 \vec{k} \\
\vec{r}(t) & =(\frac{1}{2} t^{2}+\frac{\sqrt{3}}{3} t+1) \vec{i}+(t^{2}-\frac{\sqrt{3}}{3} t) \vec{j}+(\frac{1}{2} t^{2}+\frac{5\sqrt{3}}{3} t-2) \vec{k}
\end{aligned}
$$

## 八

$\Rightarrow \lim\limits_{(x, y) \rightarrow(0,0)} f(x, y)=\lim\limits_{(x, y) \rightarrow(0,0)} \frac{\sin (x^{3}+y^{2})}{x^{2}+y^{2}}=\lim\limits_{(x, y) \rightarrow(0,0)} \frac{\sin (x^{3}+y^{2})}{x^{3}+y^{2}} \cdot \frac{x^{3}+y^{2}}{x^{2}+y^{2}}=\lim\limits_{(x, y) \rightarrow(0,0)} \frac{x^{3}+y^{2}}{x^{2}+y^{2}}$

Using polar coordinates: $x=r\cos\theta, y=r\sin\theta$:

$=\lim\limits_{r \rightarrow 0} \frac{r^{3} \cos ^{3} \theta+r^{2} \sin ^{2} \theta}{r^{2}}=\lim\limits_{r \rightarrow 0} r(\cos ^{3} \theta+ \sin ^{3} \theta)=0$

or

$0 \leq\left|\frac{x^{3}+y^{2}}{x^{2}+y^{2}}\right| =\left|\frac{x \cdot x^{2}}{x^{2}+y^{2}}+\frac{y^{2}}{x^{2}+y^{2}}\right| = | x \times \frac{x^{2}}{x^{2}+y^{2}} + y \times \frac{y^{2}}{x^{2}+y^{2}} | \leq |x|+ |y|$

$\lim\limits_{(x,y) \rightarrow (0,0)}(|x| + |y|) = 0$

$\Rightarrow \lim\limits_{(x,y) \rightarrow (0,0)}(|\frac{x^3+y^3}{x^2+y^2}|) = 0$

$\Rightarrow \lim\limits_{(x,y) \rightarrow (0,0)}(\frac{x^3+y^3}{x^2+y^2}) = 0$

$\Rightarrow \lim\limits_{(x,y) \rightarrow (0,0)}f(x,y) = 0 = f(0,0)$

$f(x,y)$ is continuous at $(0,0)$

## 九

$\Rightarrow \frac{\partial z}{\partial x}=f^{\prime}(e^{x} y) \cdot e^{x} y, \quad \frac{\partial z}{\partial y}=f^{\prime}(e^{x} y) e^{x}$

$\Rightarrow \frac{\partial z}{\partial x}+y \frac{\partial z}{\partial y}= 2 f^{\prime}(e^{x} y) e^{x} y=1$

Let $u=e^{x} y$

$\Rightarrow 2 f^{\prime}(u) u=1 \Rightarrow \frac{d f}{d u}=\frac{1}{2 u} \Rightarrow f(u)=\frac{1}{2} \ln (u)+c$

$f(1)=0 \Rightarrow \frac{1}{2} \ln 1+c=0 \Rightarrow c=0$

$\Rightarrow f(u)=\frac{1}{2} \ln |u|$

## 十

$$
\begin{aligned}
\Rightarrow f^{\prime}(x) &=\frac{1+\frac{x}{\sqrt{x^{2}+1}}}{x+\sqrt{x^{2}+1}}=\frac{\frac{\sqrt{x^{2}+1}+x}{\sqrt{x^{2}+1}}}{x+\sqrt{x^{2}+1}}=\frac{1}{\sqrt{x^{2}+1}}=(1+x^{2})^{-\frac{1}{2}} \\
&=1+\sum \limits_{k=1}^{\infty}\binom{-\frac{1}{2}}{k} x^{2 k},-1<x<1 \\
\Rightarrow f(x) & = x+\sum \limits_{k=1}^{\infty} \frac{1}{2 k+1}\binom{-\frac{1}{2}}{k} x^{2 k+1},-1<x<1
\end{aligned}
$$
