# 2020春高数下期末试题-答案

## 一

$T T T$

## 二

$D A B$

## 三

### 3-（1）

$x-y+2 z= \pm 3$

解：

$$
\begin{aligned}
& \begin{array}{l}
\text { 设 } x-y+2 z=a . \\
\nabla \vec{f}=(2 x,-4 y, 2 z) \\
\vec{n}=(1,-1,2) \\
\left\{
\begin{array} { l }
{ 2 c x = 1 } \\
{ - 4 c y = - 1 } \\
{ 2 c z = 2 }
\end{array} \Rightarrow \left\{
\begin{array}{l}
x=\frac{1}{2 c} \\
y=\frac{1}{4 c} \\
z=\frac{1}{c}
\end{array}\right.\right. \\
x^{2}-2 y^{2}+z^{2}=2 \\
\therefore \frac{9}{8 c^{2}}=2 \quad c= \pm \frac{3}{4}
\end{array}
\end{aligned}
$$

代入 $x-y+2 z$ 解得 $a= \pm 3$ !

### 3-（2）

$d x-d y$

### 3-（3）

$y+z=3$

### 3-（4）

0

## 四

$\quad 3 \sin \theta=1+\sin \theta \quad \therefore \sin \theta=\frac{\phi}{2} \quad \theta=\frac{\pi}{6} \quad \theta=\frac{\pi}{6}$

$$
A=\int_{\frac{\pi}{6}}^{\frac{5 \pi}{6}} \frac{1}{2}\left(r_{1}^{2}-r_{2}^{2}\right) d \theta=\int_{\frac{\pi}{6}}^{\frac{\pi}{6}} \frac{1}{2}\left((3 \sin \theta)^{2}-(1+\sin \theta)^{2}\right) d \theta=\pi
$$

## 五

$\int|\vec{v}| d t$

$$
\begin{aligned}
& \vec{r}(t)=(12 \sin t) \vec{i}-(12 \cos t) \vec{j}+5 t \vec{k} \\
& \vec{v}(t)=12 \cos t \vec{i}+12 \sin t \vec{j}+5 \vec{k} \\
& |\vec{v}(t)|=13
\end{aligned}
$$

$A(0,-12,0) \Rightarrow t=0$

$$
\begin{aligned}
& \left|\int_{0}^{x} 13 d t\right|=26 \pi \Rightarrow x= \pm 2 \pi \\
& \therefore(0,-12, \pm 10 \pi)
\end{aligned}
$$

## 六

$$
\lim\limits_{n \rightarrow \infty} \sqrt[n]{\left|a_{n}\right|}=|2 x|<1 \quad x \in\left(-\frac{1}{2}, \frac{1}{2}\right)
$$

（1）$x=-\frac{1}{2} \quad a_{n}=\frac{(-1)^{n}}{\ln (n+2)} \quad \because \lim\limits_{n \rightarrow \infty} \frac{1}{\ln (n+2)}=0 \quad A \quad \frac{1}{\ln (n+2)} \geqslant \frac{1}{\ln (n+2+1)}$

$\therefore \sum_{n=0}^{\infty}\frac{(-1)^{n}}{\ln (n+2)}$ 收敛 $\left|a_{n}\right|=\frac{1}{\ln (n+2)}>\frac{1}{n} \quad \therefore \sum_{n=0}^{\infty} \frac{(-1)^{n}}{\ln (n+2)}$ 条件收敛。

（2）$x=\frac{1}{2} \quad a_{n}=\frac{1}{\ln (n+2)}$＊$\sum_{n=0}^{\infty} \frac{1}{\ln (n+2)}$ 发散

$\therefore [-\frac{1}{2}, \frac{1}{2})$ 收敛

## 七

用泰勒展开和二项级数定理分别展开 $\cos (\sin x)$ 与 $\sqrt{1-x^{2}}$ 。

$\cos (\sin x)-\sqrt{1-x^{2}}=\frac{1}{3} x^{4}+O\left(x^{5}\right) \quad$（注若令 $\cos (\sin x)=1$ 则会丢掉一些, 会得出错误结论）

$$
\therefore \quad a=4 \quad b=\frac{1}{3}
$$

是错的。

## 八

内部: $f(x, y)=e^{-x^{2}-y^{2}}\left(x^{2}+2 y^{2}\right)$

$$
\begin{aligned}
& \left\{\begin{array}{l}
\frac{\partial f}{\partial x}=2 x e^{-x^{2}-y^{2}}\left(1-x^{2}-2 y^{2}\right)=0 \\
\frac{\partial f}{\partial y}=2 y e^{-x^{2}-y^{2}}\left(2-x^{2}-2 y^{2}\right)=0
\end{array}\right. \\
& \left\{\begin{array} { l }
{ x = 0 } \\
{ y = 0 }
\end{array} \left\{\begin{array}{l}
x=0 \\
y=1
\end{array} \quad \begin{array}{l}
x= \pm 1 \\
y=0
\end{array}\right.\right.
\end{aligned}
$$

外部:

$$
\begin{aligned}
& x^{2}+y^{2}=4 \quad f(x, y)=e^{-4}\left(4+y^{2}\right) \\
& \therefore( \pm 2,0)(0, \pm 2) \\
& f(0,0)=0 \quad f(0, \pm 1)=2 e^{-1} \\
& f(\pm 1,0)=e^{-1} \quad f( \pm 2,0)=4 e^{-4} \\
& f(0, \pm 2)=8 e^{-4} \quad  \\
& f_{\text {max }}=2 e^{-1} \\
& f_{\text {min }}=0
\end{aligned}
$$

## 九

$$
\begin{aligned}
& z=1 \quad z=\sqrt{x^{2}+y^{2}} \\
& x=\rho \sin \varphi \cos \theta \\
& y=\rho \sin \varphi \sin \theta \\
& z=\rho \cos  \therefore z=1 \quad \therefore \rho=\frac{1}{\cos \varphi} \\
& \int_{0}^{2 \pi} \int_{0}^{\frac{\pi}{4}} \int_{0}^{\frac{1}{\cos \varphi}} \rho \cos \varphi \rho \cdot \rho^{2} \sin \varphi d \rho d \varphi d \theta \\
& =\frac{2 \pi}{15}(2 \sqrt{2}-1) \\
\end{aligned}
$$

## 十

$$
\begin{aligned}
& \int_{L} \sin 2 x d x+2\left(x^{2}-1\right) y d y \\
& =\int_{0}^{\pi} \sin 2 x d x+2\left(x^{2}-1\right) \sin x \cos x d x\binom{y=\sin x}{d y=\cos x d x} \\
& =\int_{0}^{\pi} x^{2} \sin 2 x d x \quad \text { ( 分步积分) } \\
& =-\frac{\pi^{2}}{2} .
\end{aligned}
$$

## 十一

$\nabla \times \vec{F}=\left|\begin{array}{ccc}\vec{i} & \vec{j} & \vec{k} \\ \frac{\partial}{\partial x} & \frac{\partial}{\partial y} & \frac{0}{\partial z} \\ y & x z & x^2\end{array}\right|=(-x) \vec{i}+(-2 x) \vec{j}+(z-1) \vec{k}$.

$\vec{n}=\frac{1}{\sqrt{3}}(1,1,1)$

$d \sigma=\sqrt{1+1+1} d x d y=\sqrt{3} d x d y$

$$
\therefore \iint_{s} \nabla \times \vec{f} \cdot \vec{n} d \sigma=\int_{0}^{1} \int_{0}^{1-x}(-4 x-y) d y d x=-\frac{5}{6}
$$

## 十二

$$
\begin{aligned}
& \quad \cdot \vec{F}=2(x+y+z) \\
& \int_{0}^{\pi} \int_{0}^{2} \int_{0}^{1} 2(r \cos \theta+r \sin \theta+z) d z r d r d \theta \\
& =\int_{0}^{2 \pi} \int_{0}^{2}(2 r(\cos \theta+\sin \theta)+1) r d r d \theta\\
& =\int_{0}^{2 \pi} \int_{0}^{2}\left(2 r^{2} \cos \theta+2 r^{2} \sin \theta+r\right) d r d \theta=4 \pi
\end{aligned}
$$
