# 2022 高数下期末

> Co-Authored-By: 2208 许国祥

## 一

### 1-(1)

$D$

$\lim\limits_{n \rightarrow \infty}\left|\frac{1}{n^{\frac{1}{n}} \cdot 3}\right|=\frac{1}{3} . \quad x \in[-3,3)$

### 1-(2)

$D$

$\left.\frac{\partial f}{\partial x}\right|_{(0,0)}=\lim\limits_{x \rightarrow 0} \frac{0-0}{x}=0,\left.\frac{\partial f}{\partial y}\right|_{(0,0)} \lim\limits_{y \rightarrow 0} \frac{y^{2} \sin \frac{1}{y^{2}}-0}{y}=\lim\limits_{y \rightarrow 0} y \sin \frac{1}{y^{2}}=0$

$\frac{\partial f}{\partial x}=y^{2} \cdot \frac{-2 x}{\left(x^{2}+y^{2}\right)^{2}} \cdot \cos \left(\frac{1}{x^{2}+y^{2}}\right) \cdot \lim\limits_{(x, y \rightarrow 0,0)} \frac{\partial f}{\partial x} \neq 0$, 不连续

### 1-(3)

$C$

### 1-(4)

$B$

### 1-(5)

$B$

$\left\{\begin{array}{l}0 \leq y \leq 1 \\ y \leq x \leq 1\end{array} \Rightarrow 0 \leq y \leq x \leq 1 \Rightarrow \int_{0}^{1} \int_{0}^{x} \frac{\cos x}{x} d y d x\right.$

$$
=\int_{0}^{1} \cos x d x=\sin 1
$$

## 二

### 2-(1)

先代入 $x=5$, 得: $z^{2}+2 z-2 y^{2}=0$

$$
\frac{\partial z}{\partial y}=\frac{-F_{y}}{F_{z}}=\frac{4 y}{2 z+2}=\frac{4}{3}
$$

### 2-(2)

原式 $=\lim\limits_{(x, y) \rightarrow(0,0)} \frac{x y^{2}}{x^{2}+y^{2}} \leq \lim\limits_{(x, y) \rightarrow(0,0)} x=0$

又, 原式 $>0$, 故原式 $=0$

### 2-(3)

$=\int_{0}^{2 \pi} \int_{0}^{1} e^{-r^{2}} \cdot r d r d \theta=\int_{0}^{2 \pi} \frac{1}{2}\left(1-\frac{1}{e}\right) d \theta=\pi\left(1-\frac{1}{e}\right)$

### 2-(4)

$\frac{2}{3} a^{3} \pi$

### 2-(5)

保守场: $\frac{\partial f}{\partial x}=y z e^{x z}, f=y e^{x z}+g(y, z), \frac{\partial f}{\partial y}=e^{x z}+\frac{\partial g}{\partial y}$

$$
\frac{\partial g}{\partial y}=0 \Rightarrow f=y e^{x z}+h(z), \frac{\partial f}{\partial z}=x y e^{x z}+h^{\prime}(z), \quad h(z)=C, \Rightarrow f=y e^{x z}+C
$$

代入, 得:  $4 \cdot e^{0}-1 \cdot e^{0}=3$

## 三

$\quad l_{1}$ 方向向量: $\vec{v}_{1}=\langle0,1,1\rangle, l_{2}$ 方向向量 $\vec{v}_{2}=\langle1,2,1\rangle$

$\vec{n}=\vec{v}_{1} \times \vec{v}_{2}=\left|\begin{array}{lll}\hat{i} & \hat{j} & \hat{k} \\ 0 & 1 & 1 \\ 1 & 2 & 1\end{array}\right|=\hat{i}+\hat{j}-\hat{k}-2 \hat{i}=\langle-1,1,-1\rangle$

$\Rightarrow$ 平面方程: $-x+y-z=0$

## 四

原试 $=\lim\limits_{n \rightarrow \infty} n^{3}\left(\frac{2}{n}-\frac{1}{3!} \cdot\left(\frac{2}{n}\right)^{3}+\cdots\right)-2 n^{2}$

$$
=\lim\limits_{n \rightarrow \infty} 2 x^{2}-\frac{8}{3!}-2 n^{2}=-\frac{4}{3}
$$

## 五

$\quad \nabla f=(y) \hat{i}+\left.(x+2 y) \hat{j} \quad \nabla f\right|_{(3,2)}=2 \hat{i}+7 \hat{j}$

又有且仅有 $\langle-7,2\rangle$ 或 $\langle 7,-2\rangle$ 所在方向的向量为 $\left.\nabla f\right|_{(3,2)}$

内积为 0,

故:

+ 方向 $1: \vec{v}_{1}=\left\langle\frac{-7}{\sqrt{53}}, ~ \frac{2}{\sqrt{53}}\right\rangle$ 所在方向,
+ 方向 $2: \vec{v}_{2}=\left\langle\frac{7}{\sqrt{53}}, ~ \frac{-2}{\sqrt{53}}\right\rangle$ 所在方向

## 六

$D:(x-1)^{2}+(y-1)^{2}=2$ 令 $v=x-1, \quad u=y-1, \quad J=\left|\frac{\partial(x, y)}{\partial(v, w)}\right|=1$

原式 =

$$
\begin{aligned}
& \iint_{G}(v+1)(u+1) d A=\int_{0}^{2 \pi} \int_{0}^{\sqrt{2}}\left(r^{2} \sin \theta \cos \theta+r \sin \theta+r \cos \theta+1\right) r d r d \theta \\
& =\int_{0}^{2 \pi}\left[\frac{1}{4} r^{4} \sin \theta \cos \theta+\frac{1}{3} r^{3}(\sin \theta+\cos \theta)+\frac{1}{2} r^{2}\right]_{0}^{\sqrt{2}} d \theta \\
& =\int_{0}^{2 \pi} d \theta=2 \pi
\end{aligned}
$$

## 七

令 $\sqrt{x^{2}+y^{2}}=\sqrt{1-x^{2}-y^{2}}, \Rightarrow x^{2}+y^{2}=\frac{1}{2}$

$$
\begin{aligned}
& M=\iiint_{R} d V=\int_{0}^{2 \pi} \int_{0}^{\frac{1}{\sqrt{2}}} \int_{r}^{\sqrt{1-r^{2}}} r d z d r d \theta=\int_{0}^{2 \pi} \int_{0}^{\frac{1}{2}} r \sqrt{1-r^{2}}-r^{2} d r d \theta \\
& =\int_{0}^{2 \pi} \left[-\frac{1}{3}\left(1-r^{2}\right)^{\frac{3}{2}}-\frac{1}{3} r^{3}\right]_{0}^{\frac{1}{\sqrt{2}}} d \theta=\int_{0}^{2 \pi} \frac{1}{3}-\frac{1}{3 \sqrt{2}} d \theta=\left(\frac{1}{3}-\frac{1}{3 \sqrt{2}}\right) 2 \pi \\
& M_{x y}=\int_{0}^{2 \pi} \int_{0}^{\frac{1}{\sqrt{2}}} \int_{r}^{\sqrt{1 -r^{2}}} r z d z d r d \theta=\int_{0}^{2 \pi} \int_{0}^{\frac{1}{\sqrt{2}}} \frac{1}{2} r\left(1-2 r^{2}\right) d r d \theta
\end{aligned}
$$

$=\int_{0}^{2 \pi}\left[\frac{1}{4} r^{2}-\frac{1}{4} r^{4}\right]_{0}^{\frac{1}{\sqrt{2}}} d \theta=\int_{0}^{2 \pi} \frac{1}{16} d \theta=\frac{\pi}{8}$

$\Rightarrow \bar{z}=\frac{9 \sqrt{2}}{48(\sqrt{2}-1)}$

由对称性, 得 $\bar{x}=\bar{y}=0$

故: 形心为 $\left(0,0, \frac{9 \sqrt{2}}{48(\sqrt{2}-1)}\right)$

## 八

$\oint_{c} \vec{F} \cdot d \vec{r}=\iint_{s} \nabla \times \vec{F} \cdot \vec{n} d \sigma=0$

## 九

### 9-(i)

在 $x^{2}+y^{2}=1$ 上

令 $g(x, y)=x^{2}+y^{2}-1=0$

$\nabla f=\lambda \nabla g, \Rightarrow(6 x+4 y) \hat{i}+4 x \hat{\jmath}=\lambda[(2 x) \hat{\imath}+2 y \hat{\jmath}]$

$$
\begin{aligned}
\Rightarrow \left\{
\begin{array}{l}
6 x+4 y=2 \lambda x  \\
4 x=2 \lambda y
\end{array} \right
\end{aligned}
$$

$\Rightarrow 3 \lambda+4=\lambda^{2}, \lambda=4 \text { 或 } \lambda=-1$

+ $\lambda=4, \Rightarrow y= \pm \frac{1}{\sqrt{5}}, x= \pm \frac{2}{\sqrt{5}}$
+ $\lambda=-1, \Rightarrow y= \pm \frac{2}{\sqrt{5}}, x=-\frac{1}{\sqrt{5}}$

取 $\left\{\begin{array}{l}y=\frac{1}{\sqrt{5}} \\ x=\frac{2}{\sqrt{5}}\end{array}\right.$ 代 $\lambda, f=\frac{12}{5}+\frac{8}{5}=4$

取 $\left\{\begin{array}{l}y=\frac{2}{\sqrt{5}} \\ x=-\frac{1}{\sqrt{5}}\end{array}\right.$ 代 $\lambda, f=-1$

### 9-(ii)

$\frac{\partial f}{\partial x}=6 x+4 y, \frac{\partial f}{\partial y}=4 x$, 当 $f_{x}=f_{y}=0$ 时, $x=y=0$

此时 $f=0 \quad f_{x x}=6>0$,

$f_{y y}=0, f_{x y}=4, \quad f_{x x} f_{y y}-f_{x y}^{2}<0, \Rightarrow$ 是 saddle point

综上所述

+ 最大值在 $\left(\frac{1}{\sqrt{5}}, ~ \frac{2}{\sqrt{5}}\right)$ 和 $\left(\frac{-1}{\sqrt{5}}, ~-\frac{2}{\sqrt{5}}\right)$ 处取得, 为4,
+ 最小值在 $\left(\frac{-1}{\sqrt{5}}, \frac{2}{\sqrt{5}}\right)$ 和 $\left(\frac{1}{\sqrt{5}}, ~-\frac{2}{\sqrt{5}}\right)$ 处取得, 为-1
