i～3 FTF

动 ${ }^{\prime} B D D C D$ ．

三．（1）$\frac{1}{2}$（2）（0，1）（3） $\ln (\sec 1)$

四．（1） $\lim _{n \rightarrow \infty} \sqrt[n]{\left|a_{n}\right|}=(x-1)^{2}<1$

$$
x \in(0,2)
$$

Q $\quad x=0 \quad a_{n}=\frac{(-1)^{n+1}}{\sqrt{n+9012} \ln n}$ ．

$\left|a_{n}\right|$ 单减。

旦 $\frac{\left|a_{n}\right|}{n \ln x}=\infty \quad \sum \frac{1}{n \ln n}$ 发散

$\therefore$ 条件收敛。

（2）$x=2 \quad a_{n}=\frac{(-1)^{n}}{\sqrt{n+9912} \ln n}$

13 上

（2）绝对收敛（0，2）

条件收登文 $x=0, ~ x=2$

五，

$$
\begin{aligned}
& \text { (1) } \int_{0}^{2 \pi} \int_{0}^{\frac{\sqrt{2}}{2}} \int_{r}^{\sqrt{1-r^{2}}}(r \cos \theta+z) r d z d r d \theta \\
& \text { (2) } \int_{0}^{2 \pi} \int_{0}^{\frac{\pi}{4}} \int_{0}^{1}(\rho \sin \varphi \cos \theta+\rho \cos \varphi) \rho^{2} \sin \varphi d \rho d \varphi d \theta
\end{aligned}
$$

六：$\quad V=8 x y z$

$$
\begin{aligned}
& g(x, y, z)=\frac{x^{2}}{a^{2}}+\frac{y^{2}}{b^{2}}+\frac{z^{2}}{c^{2}}=1 \\
& \nabla \vec{V}=\lambda \nabla \vec{g} \\
& \begin{cases}8 y z=\lambda \frac{2 x}{a^{2}} & \text { (0) } \lambda=0 \text { 不成立 } \\
8 x z=\lambda \frac{2 y}{b^{2}} & \text { (2 } \lambda \neq 0 \\
8 x y=\lambda \frac{2 z}{c^{2}} & \frac{x^{2}}{a^{2}}=\frac{y^{2}}{b^{2}}=\frac{z^{2}}{c^{2}} \Rightarrow x=\frac{a}{\sqrt{3}} y=\frac{b}{\sqrt{3}} z=\frac{c}{\sqrt{3}}\end{cases} \\
& \therefore V=\frac{8 a b c}{3 \sqrt{3}}
\end{aligned}
$$

t：

$$
\begin{aligned}
& y=x^{2} \quad x=1 \\
& \vec{r}(t)=\left(t, t^{2}\right) \\
& \vec{V}(t)=(1,2 t) \\
& |\vec{V}(t)|=\sqrt{4 t^{2}+1} \\
& \vec{T}=\left(\frac{1}{\sqrt{4 t^{2}+1}}, \frac{2 t}{\sqrt{4 t^{2}+1}}\right)
\end{aligned}
$$

$$
\begin{gathered}
\frac{d \vec{T}}{d t}=\left(-\frac{4 t}{(1+4)^{3 / 2}}, \frac{2}{\left(1+4 t^{2}\right)^{\frac{3}{2}}}\right) \\
k(1)=\frac{2}{5 \sqrt{5}} \quad r=\frac{5 \sqrt{5}}{2} \\
(1,1)+\frac{5 \sqrt{5}}{2} \cdot \frac{1}{\sqrt{5}}(-2,1)=\left(-4, \frac{7}{2}\right) \\
\therefore(x+4)^{2}+\left(y-\frac{7}{2}\right)^{2}=\frac{125}{4}
\end{gathered}
$$

$$
\begin{aligned}
& \therefore M \\
&=\int_{0}^{2} \int_{0}^{\sqrt{x}} \int_{0}^{4-x^{2}} x y d z d y d x=\frac{32}{15} \\
& M_{x y}=\frac{256}{105} \\
& M_{y z}=\frac{8}{3} \\
& M_{x z}=\frac{256 \sqrt{2}}{231} \\
& \therefore \bar{x}=\frac{M_{y z}}{M}=\frac{5}{4} \quad \bar{y}=\frac{M_{x z}}{M}=\frac{40 \sqrt{2}}{77} \quad \bar{z}=\frac{M_{x y}}{M}=\frac{8}{7} .
\end{aligned}
$$

九

$$
\begin{array}{ll}
\left.\begin{array}{l}
\begin{array}{l}
u=y-x \\
v=y+x
\end{array} \\
\left.\begin{array}{ll}
\begin{array}{l}
x=0 \\
y=0 \\
x+y=2
\end{array} & \left.v=\left|\begin{array}{cc}
-\frac{1}{2} & \frac{1}{2} \\
\frac{1}{2} & \frac{1}{2}
\end{array}\right| \right\rvert\,=\frac{1}{2} \\
I=\int_{0}^{2} \int_{-v}^{v} e^{\frac{u}{v}} \cdot \frac{1}{2} d u d v=e-e^{-1}
\end{array}\right\} \quad \uparrow^{v}
\end{array}\right\}=u
\end{array}
$$

t．（1）$\frac{\partial P}{\partial y}=\frac{\partial N}{\partial z} ; \frac{\partial P}{\partial x}=\frac{\partial M}{\partial z} ; \frac{\partial N}{\partial x}=\frac{\partial M}{\partial y}$

$$
\therefore \text { exact }
$$

（2）

$$
\begin{aligned}
& \frac{\partial f}{\partial x}=e^{x} \ln y \\
& t=e^{x} \ln y+g(y, z) \\
& \frac{\partial f}{\partial z}=y \cos z \quad \therefore f=e^{x} \ln y+y \sin z+h(y) \\
& \frac{\partial f}{\partial y}=\frac{e^{x}}{y}+\sin z+\frac{\partial h}{\partial z} \quad \therefore \frac{\partial h}{\partial z}=c \\
& \therefore f=e^{x} \ln y+y \sin z+c \\
& f(1,3, \pi)-f(1,1,1)=e \ln 3-\sin 1
\end{aligned}
$$

t－

$$
\begin{aligned}
& \nabla \cdot(4 \times \vec{j})=\left|\begin{array}{ccc}
\vec{i} & \vec{j} & \vec{k} \\
\frac{\partial}{\partial x} & \frac{j}{\partial y} & \frac{\delta}{d z} \\
0 \cdot & 4 x & 0
\end{array}\right|=4 \vec{k} \\
& \therefore \quad \int_{s} \nabla \times(4 \times \vec{j}) \cdot \vec{r} d \sigma=\iint_{s} 4 \vec{k} \cdot \vec{k} d \sigma=4 \int_{s} d \sigma=64 \pi
\end{aligned}
$$

$十$ 二，$\nabla \cdot \vec{F}=6+4 y \quad$ stocks＇定理．

$$
\begin{aligned}
\iiint_{v}(6+4 y) d v & =\int_{0}^{1} \int_{0}^{\sqrt{1-x^{2}}} \int_{0}^{\sqrt{x^{2} \theta^{2}}}(6+4 y) d z d y d x \\
& =\int_{0}^{\frac{\pi}{2}} \int_{0}^{1} \int_{0}^{r}(6+4 r \sin \theta) r d z d r d \theta \\
& =\pi+1
\end{aligned}
$$

$$
\begin{aligned}
&+\equiv, \quad \cos a_{n}-a_{n}=\cos b_{n} \\
& \cos a_{n}-\cos b_{n}=a_{n}>0 \\
& \Rightarrow 0<a_{n}<b_{n} \\
& \sum_{n=1}^{\infty} b_{n} \text { 收敛 } \Rightarrow \lim _{n \rightarrow \infty} b_{n}=0 \\
& 0 \leqslant \lim _{n \rightarrow \infty} a_{n} \leq b_{n} \quad \therefore \lim _{n \rightarrow \infty} a_{n}=0 .
\end{aligned}
$$

